<?xml version="1.0" encoding="UTF-8"?>

<section xml:id="sec-proof-1" xmlns:xi="http://www.w3.org/2001/XInclude">
  <title>Proof of Dirichlet's theorem, part 1</title>

  <introduction>
  <p>
  In this section we'll start to prove Dirichlet's theorem.
  We'll give essentially the whole proof except for
  the hardest part of the proof,
  showing that <m>L(1,\chi) \neq 0</m> for every character <m>\chi</m>.
  Showing that will be the second part of the proof,
  in the next section of notes.
  </p>
  
  <p>
  As in the statement of Dirichlet's theorem,
  we fix positive integers <m>a,q</m>
  such that <m>(a,q) = 1</m>.
  </p>
  
  </introduction>
  
  <subsection>
  <title> Going from summing over primes to summing over an arithmetic progression </title>
  
  <proposition>
  <title> Step 1 </title>
  
  <statement>
  <men>
    \sum_{p \leq x, p \equiv a \pmod{q}} \frac{\log p}{p}
    = \sum_{n \leq x, n \equiv a \pmod{q}} \frac{\Lambda(n)}{n} + O(1)
  </men>.
  </statement>
  
  <proof>
  <p>
  We have
  <mdn>
  <mrow> \sum_{n \leq x, n \equiv a \pmod{q}} \frac{\Lambda(n)}{n}
    \amp = \sum_{p^k \leq x, p^k \equiv a \pmod{q}} \frac{\log p}{p^k} </mrow>
  <mrow> \amp = \sum_{p \leq x, p \equiv a \pmod{q}} \frac{\log p}{p}
    + \sum_{p^k \leq x, k \geq 2, p^k \equiv a \pmod{q}} \frac{\log p}{p^k} . </mrow>
  </mdn>
  The last sum converges: we have
  <mdn>
  <mrow> \sum_{p^k \leq x, k \geq 2, p^k \equiv a \pmod{q}} \frac{\log p}{p^k}
    \amp \leq \sum_n \log n \sum_{k \geq 2} \frac{1}{n^k} </mrow>
  <mrow> \amp = \sum_n \frac{\log n}{n(n-1)} </mrow>
  </mdn>
  which converges by comparison with a p-series.
  </p>
  </proof>
  </proposition>
  
  </subsection>
  
  <subsection>
  <title> Summing over all positive integers by using the orthogonality relations of Dirichlet characters </title>
  
  <p>
  Our next step is to take the sum of <m>\frac{\Lambda(n)}{n}</m>
  from a sum over <m>n \equiv a \pmod{q}</m>
  into a sum over all positive <m>n</m>.
  We will use the orthogonality relations of Dirichlet characters
  so that the terms <m>n \equiv a \pmod{q}</m> remain in the sum,
  while all other values of <m>n</m> cancel out, up to some bounded quantity.
  </p>
  
  <proposition>
  <title> Step 2 </title>
  
  <statement>
  We have
  <men>
    \sum_{n \leq x, n \equiv a \pmod{q}} \frac{\Lambda(n)}{n}
    = \frac{1}{\phi(q)} \sum_{\chi \mod q} \overline{\chi}(a) \sum_{n \leq x} \frac{\chi(n) \Lambda(n)}{n}
  </men>.
  In addition, for the principal character,
  <men>
    \sum_{n \leq x} \frac{\chi_0(n) \Lambda(n)}{n} = \log x + O(1)
  </men>.
  Hence
  <men>
    \sum_{n \leq x, n \equiv a \pmod{q}} \frac{\Lambda(n)}{n}
    = \frac{1}{\phi(q)} \log x
    + \frac{1}{\phi(q)} \sum_{\chi \mod q, \chi \neq \chi_0} \overline{\chi}(a) \sum_{n \leq x} \frac{\chi(n) \Lambda(n)}{n}
    + O(1)
  </men>.
  </statement>
  
  <proof>
  <p>
  Recall that for any integers <m>k,m</m>, if <m>(m,q)=1</m>,
  we have the orthogonality relation
  <me>
    \sum_{\chi \mod q} \chi(k) \overline{\chi}(m) =
    \begin{cases}
      \phi(q), \amp \text{if } k \equiv m \pmod{q}, \\
      0, \amp \text{otherwise}.
    \end{cases}
  </me>
  Using this,
  <mdn>
  <mrow> \sum_{n \leq x, n \equiv a \pmod{q}} \frac{\Lambda(n)}{n}
    \amp = \sum_{n \leq x} \frac{\Lambda(n)}{n}
      \left( \frac{1}{\phi(q)} \sum_{\chi \mod q} \chi(n) \overline{\chi}(a) \right) </mrow>
  <mrow> \amp = \frac{1}{\phi(q)} \sum_{\chi \mod q} \overline{\chi}(a) \sum_{n \leq x} \frac{\chi(n)\Lambda(n)}{n} . </mrow>
  </mdn>
  This shows the first claim.
  </p>
  
  <p>
  For the principal character, the summation of
  <m> \frac{\chi_0(n)\Lambda(n)}{n} </m>
  agrees with the summation of <m> \frac{\Lambda(n)}{n} </m>
  except for terms where <m>(n,q) \gt 1</m>.
  Mertens's theorem includes the result that
  <me>
    \sum_{n \leq x} \frac{\Lambda(n)}{n} = \log x + O(1)
  </me>.
  Now consider the terms with <m>(n,q) \gt 1</m>.
  There is an additional restriction: <m>\Lambda(n) \neq 0</m>
  only when <m>n = p^k</m> is a power of a prime.
  So the difference between the sum we are considering,
  and the sum that appeared in Mertens's theorem,
  is just for terms where <m>n = p^k</m> is a power of a prime,
  for a prime <m>p</m> that divides the modulus <m>q</m>.
  </p>
  
  <p>
  There are only finitely many such primes.
  Each such prime <m>p</m> contributes a difference of
  <m>\sum_{p^k \leq x} \frac{\log p}{p^k}</m>.
  We have seen already the convergence of the full series
  <me>
    \sum_{k=1}^{\infty} \frac{\log p}{p^k}
  </me>.
  So the sum for <m>p^k \leq x</m> is a bounded amount.
  Adding up these bounded amounts for the finitely many primes
  that divide <m>q</m> gives a bounded amount,
  in other words an <m>O(1)</m>.
  This proves the second claim.
  </p>
  
  <p>
  The third claim follows from the first one,
  separating out the terms for the principal and nonprincipal characters,
  and substituting the estimate for the principal character.
  </p>
  
  </proof>
  </proposition>
  
  <p>
  Combining this with step 1, we get
  <me>
    \sum_{p \leq x, p \equiv a \pmod{q}} \frac{\log p}{p}
    = \frac{1}{\phi(q)} \log x
    + \frac{1}{\phi(q)} \sum_{\chi \mod q, \chi \neq \chi_0} \overline{\chi}(a) \sum_{n \leq x} \frac{\chi(n) \Lambda(n)}{n}
    + O(1)
  </me>.
  Our goal is to show that it is equal to
  <m>\frac{1}{\phi(q)} \log x + O(1)</m>.
  So, what is left is to show that the middle term is bounded (<m>O(1)</m>).
  In fact we will show that for each <m>\chi \neq \chi_0</m>,
  the sum
  <m> \sum_{n \leq x} \frac{\chi(n)\Lambda(n)}{n} </m>
  is bounded.
  Since there are finitely many characters (<m>\hat{G}</m> is a finite group),
  then adding them all together gives a bounded quantity.
  </p>
  
  </subsection>
  
  <subsection>
  <title> Each nonprincipal character contributes a bounded amount </title>
  
  <proposition>
  <title> Step 3 </title>
  
  <statement>
  Let <m>\chi \neq \chi_0</m> be a nonprincipal character modulo <m>q</m>.
  We have
  <men>
    \sum_{n \leq x} \frac{\chi(n) \Lambda(n)}{n} =
    \begin{cases}
      O(1), \amp \text{if } L(1,\chi) \neq 0, \\
      -\log x + O(1), \amp \text{otherwise}.
    \end{cases}
  </men>
  </statement>
  
  <proof>
  <title> Proof: Nonzero case </title>
  
  <p>
  Assume that <m>L(1,\chi) \neq 0</m>.
  Consider the sum
  <me>
    \sum_{n \leq x} \frac{\chi(n)\log n}{n}
  </me>.
  By <xref ref="dirichlet-l-function-convergence-examples"/>
  this sum converges as <m>x \to \infty</m>, so it is bounded, i.e., <m>O(1)</m>.
  </p>
  
  <p>
  On the other hand, we have
  <men>
    \sum_{n \leq x} \frac{\chi(n)\log n}{n}
    = \sum_{n \leq x} \frac{\chi(n)}{n} \sum_{d \mid n} \Lambda(n)
    = \sum_{dk \leq x} \frac{\chi(dk)}{dk} \Lambda(d)
  </men>.
  The first equality follows from the identity
  <m>\log n = \sum_{d \mid n} \Lambda(d)</m> which we have seen before.
  The second equality is by substitution <m>n=dk</m>.
  </p>
  
  <p>
  Since every Dirichlet character is completely multiplicative,
  we have <m>\Lambda(dk) = \Lambda(d)\Lambda(k)</m>
  (for all <m>d,k</m>, including if <m>(d,k) \gt 1</m>).
  So the summand in the last sum can be rewritten as
  <men>
    \frac{\chi(dk)}{dk} \Lambda(d) = \frac{\chi(d)\Lambda(d)}{d} \cdot \frac{\chi(k)}{k}
  </men>.
  </p>
  
  <p>
  First we will fix <m>d</m> and evaluate the sum over <m>k \leq \frac{x}{d}</m>.
  We know that for <m>d \leq x</m>,
  <men>
    \sum_{k \leq \frac{x}{d}} \frac{\chi(k)}{k} = L(1,\chi) + O\left(\frac{d}{x}\right)
  </men>
  by <xref ref="dirichlet-l-function-convergence-examples"/>.
  Therefore
  <md>
  <mrow> \sum_{dk \leq x} \frac{\chi(d)\Lambda(d)}{d} \cdot \frac{\chi(k)}{k}
    \amp = \sum_{d \leq x} \frac{\chi(d)\Lambda(d)}{d} \cdot \left( L(1,\chi) + O\left(\frac{d}{x}\right) \right) </mrow>
  <mrow> \amp = L(1,\chi) \sum_{d \leq x} \frac{\chi(d)\Lambda(d)}{d}
      + \sum_{d \leq x} \frac{\chi(d)\Lambda(d)}{d} \cdot O\left(\frac{d}{x}\right) </mrow>
  <mrow> \amp = L(1,\chi) \sum_{d \leq x} \frac{\chi(d)\Lambda(d)}{d}
      + \sum_{d \leq x} \chi(d)\Lambda(d) \cdot O\left(\frac{1}{x}\right) </mrow>
  </md>
  We want to simplify that last sum.
  First, observe that we can bound the sum:
  <me>
    \left| \sum_{d \leq x} \chi(d)\Lambda(d) \right| \leq \sum_{d \leq x} |\Lambda(d)| = \sum_{d \leq x} \Lambda(d)
  </me>.
  Here we are using that <m>|\chi(d)| \leq 1</m>
  because each <m>\chi(d)</m> is a root of unity, or zero.
  Every value of <m>\Lambda(d)</m> is either <m>\log p</m> or zero;
  and <m>\log p \gt 0</m> (we have <m>\log 2 \lt 1</m>, but still <m>\gt 0</m>).
  Recall that <m>\sum_{d \leq x} \Lambda(d) = \psi(x)</m>,
  Chebyshev's <m>\psi</m> function, by definition.
  And recall that by Chebyshev's estimates, <m>\psi(x) = O(x)</m>.
  </p>
  
  <p>
  So, <m>\sum_{d \leq x} \chi(d)\Lambda(d) = O(x)</m>.
  Can we conclude that <m>\sum_{d \leq x} \chi(d)\Lambda(d)O(\frac{1}{x}) = O(1)</m>?
  Not immediately.
  The problem is that the implicit constant appearing in the <m>O(1/x)</m> factor
  might a priori depend on <m>d</m>; and it might grow as <m>d</m> grows.
  </p>
  
  <p>
  Well, the <m>O(1/x)</m> factors are not arbitrary, independent things.
  They come from the same place: the tails of the sum
  <m>\sum \frac{\chi(k)}{k}</m>.
  Specifically, we have
  <men>
    \left| \sum_{k \gt x} \frac{\chi(k)}{k} \right|
    \leq C \cdot \frac{1}{x}
  </men>
  for some constant <m>C</m> that doesn't depend on <m>x</m>.
  In particular that means
  <me>
    \left| \sum_{k \gt \frac{x}{d}} \frac{\chi(k)}{k} \right|
    \leq C \cdot \frac{d}{x}
  </me>
  where the constant <m>C</m> doesn't depend on <m>x</m> or on <m>d</m>.
  So, the sum we're trying to bound can now be bounded:
  <men>
    \left| \sum_{d \leq x} \frac{\chi(d)\Lambda(d)}{d} O\left(\frac{d}{x}\right) \right|
    \leq \sum_{d \leq x} \left| \frac{\chi(d)\Lambda(d)}{d} \cdot C \cdot \frac{d}{x} \right|
    \leq \frac{C}{x} \sum_{d \leq x} \Lambda(d)
  </men>
  and again, the sum of <m>\Lambda(d)</m> is equal to <m>\psi(x)</m>
  which is <m>O(x)</m>.
  </p>
  
  <p>
  In conclusion,
  <men>
    L(1,\chi) \sum_{d \leq x} \frac{\chi(d) \Lambda(d)}{d} + O(1)
    = \sum_{n \leq x} \frac{\chi(n)\Lambda(n)}{n}
    = O(1)
  </men>
  and so therefore
  <men>
    L(1,\chi) \sum_{d \leq x} \frac{\chi(d) \Lambda(d)}{d} = O(1)
  </men>
  Finally, since <m>L(1,\chi) \neq 0</m>,
  we can divide to get that the sum is <m>O(1)</m> as claimed.
  </p>

  <remark>
  <p>
  It could have all gone wrong if it had been
  <me>
    \sum_{d \leq x} \chi(d)\Lambda(d) \cdot O\left(\frac{1}{x}\right)
    = \sum_{d \leq x} \chi(d)\Lambda(d) \cdot \frac{C_d}{x}
  </me>
  with <m>C_d \to \infty</m>.
  This highlights the importance of knowing when the implicit constant
  in big O notation is dependent or independent of other variables.
  </p>
  </remark>
  </proof>
  
  
  <proof>
  <title> Proof: Zero case </title>
  
  <p>
  Assume that <m>L(1,\chi) = 0</m>.
  We will show that <m>\log x + \sum_{n \leq x} \frac{\chi(n)\Lambda(n)}{n}</m>
  is bounded.
  </p>
  
  <p>
  Recall the identities
  <me>
  	\Lambda(n) = \sum_{d \mid n} \mu(d) \log \frac{n}{d} = - \sum_{d \mid n} \mu(d) \log d
  </me>.
  (As a reminder: We have mentioned the identity <m>\log n = \sum_{d \mid n} \Lambda(d)</m>.
  Then MÃ¶bius inversion gives <m>\Lambda = \mu * \log</m>, which is the first equality.
  The second equality is algebraic simplification.)
  </p>
  
  <p>
  Using these identities,
  <mdn>
  <mrow> \sum_{d \mid n} \mu(d) \log \frac{x}{d}
  	\amp = (\log x) \sum_{d \mid n} \mu(d) - \sum_{d \mid n} \mu(d) \log d </mrow>
  <mrow> \amp = \begin{cases}
  	\log x, \amp \text{if } n = 1 \\
  	\Lambda(n), \amp \text{if } n \gt 1
  	\end{cases}
  </mrow>
  </mdn>
  because if <m>n = 1</m> then <m>\Lambda(n) = 0</m> and <m>\sum_{d \mid n} \mu(d) = 1</m>,
  while if <m>n \gt 1</m> then <m>\sum_{d \mid n} \mu(d) = 0</m>.
  </p>
  
  <p>
  Now we consider <m>\log x + \sum_{n \leq x} \frac{\chi(n) \Lambda(n)}{n}</m>,
  with the goal of showing it is bounded.
  Both of the expressions <m>\log x</m> and <m>\Lambda(n)</m> can be replaced
  with <m>\sum_{d \mid n} \mu(d) \log \frac{x}{d}</m>.
  In addition, when <m>n=1</m> we have <m>\frac{\chi(n)}{n} = \frac{\chi(1)}{1} = 1</m>.
  After we make this substitution, we will interchange the order of summation:
  <mdn>
  <mrow>
  	\log x + \sum_{n \leq x} \frac{\chi(n)\Lambda(n)}{n}
  	\amp = \sum_{n \leq x} \frac{\chi(n)}{n} \sum_{d \mid n} \mu(d) \log \frac{x}{d}
  </mrow>
  <mrow>
  	\amp = \sum_{d \leq x} \mu(d) \log \frac{x}{d} \sum_{k \leq \frac{x}{d}} \frac{\chi(dk)}{dk}
  </mrow>
  <mrow>
  	\amp = \sum_{d \leq x} \mu(d) \left( \log \frac{x}{d}\right) \frac{\chi(d)}{d} \sum_{k \leq \frac{x}{d}} \frac{\chi(k)}{k}
  </mrow>
  <mrow>
  	\amp = \sum_{d \leq x} \mu(d) \left( \log \frac{x}{d}\right) \frac{\chi(d)}{d} \left( L(1,\chi) + O\left(\frac{d}{x} \right) \right)
  </mrow>
  <mrow>
  	\amp = \sum_{d \leq x} \mu(d) \left( \log \frac{x}{d}\right) \frac{\chi(d)}{d} \cdot O\left(\frac{d}{x} \right)
  </mrow>
  <mrow>
  	\amp = O\left(\frac{1}{x}\right) \sum_{d \leq x} \mu(d) \left( \log \frac{x}{d} \right) \chi(d)
  </mrow>
  <mrow>
  	\amp = O\left(\frac{1}{x}\right) O\left(\sum_{d \leq x} \log \frac{x}{d} \right)
  </mrow>
  <mrow>
  	\amp = O(1) \quad \text{(!!) (Exercise)}
  </mrow>
  </mdn>
  Therefore <m>\sum_{n \leq x} \frac{\chi(n)\Lambda(n)}{n} = -\log x + O(1)</m>.
  </p>
  </proof>
  
  </proposition>

  </subsection>
  
</section>