<?xml version="1.0" encoding="UTF-8"?>

<section xml:id="sec-proof-2" xmlns:xi="http://www.w3.org/2001/XInclude">
  <title>Proof of Dirichlet's theorem, part 2</title>

  <introduction>
  <p>
  In this section we'll finish the proof of Dirichlet's theorem.
  What is left is to
  show that <m>L(1,\chi) \neq 0</m> for every character <m>\chi</m>.
  We already know it for the principal character <m>\chi_0</m>
  (in fact <m>L(1,\chi_0)=\infty</m>), so we just have to show it for nonprincipal characters.
  This will happen in two steps:
  First we'll show it for real nonprincipal characters.
  The Dirichlet hyperbola method makes an appearance here.
  Second, we'll show it for nonreal nonprincipal characters,
  by a clever trick which hinges on complex conjugation.
  </p>
  
  <p>
  We fix a positive integer <m>q</m>.
  For this part of the proof, the integer <m>a</m>
  (as in, the primes such that <m>p \equiv a \pmod{q}</m>)
  doesn't play a role.
  </p>
  
  </introduction>
  
  <subsection>
  <title> Real nonprincipal characters </title>
  
  <definition>
  <p>
  A character <m>\chi</m> is called <term>real</term> if its values are in the real numbers.
  </p>
  </definition>
  
  <p>
  Since the values of <m>\chi</m> are roots of unity (or zero),
  the only real values are <m>\pm 1, 0</m>.
  For example (we won't use these examples in the proof):
  <ol>
  <li> The principal character is real. </li>
  <li> If <m>q</m> is prime, the Legendre symbol <m>\chi(n) = \left(\frac{n}{q}\right)</m>
  is a real character. </li>
  <li> As an exercise, one can show that modulo a prime <m>q</m>,
  the principal character and the Legendre symbol are the only real characters. </li>
  </ol>
  </p>
	
	<theorem>
	<statement>
	Let <m>\chi</m> be a real nonprincipal Dirichlet character modulo <m>q</m>.
	Then <m>L(1,\chi) \neq 0</m>.
	</statement>
	
	<proof>
	
	<p>
	We know that <m>\chi</m> is completely multiplicative.
	</p>
	
	<claim>
	<title> Step 1 </title>
	<statement>
	<p>
	Let <m>r(n) = \sum_{d \mid n} \chi(d)</m>.
	Then <m>r(n) \geq 0</m> for all <m>n \in \bbN</m>
	and <m>r(n) \geq 1</m> if <m>n</m> is a square.
	</p>
	</statement>
	
	<proof>
	<p>
	Since <m>\chi</m> is (completely) multiplicative
	and <m>r = \chi * 1</m> (Dirichlet convolution),
	it follows that <m>r</m> is multiplicative (but not necessarily completely multiplicative).
	</p>
	
	<p>
	Let <m>p</m> be a prime and <m>a \geq 1</m>.
	Then
	<mdn>
	<mrow> r(p^a) \amp = \sum_{d \mid p^a} \chi(d) </mrow>
	<mrow> \amp = \chi(1) + \chi(p) + \chi(p^2) + \dotsb + \chi(p^a) </mrow>
	<mrow> \amp = \chi(1) + \chi(p) + \chi(p)^2 + \dotsb + \chi(p)^a </mrow>
	<mrow> \amp = \begin{cases}
		a+1, \amp \text{if } \chi(p) = 1; \\
		1, \amp \text{if } \chi(p) = 0; \\
		1, \amp \text{if } \chi(p) = -1 \text{ and } a=2k; \\
		0, \amp \text{if } \chi(p) = -1 \text{ and } a=2k+1.
		\end{cases} </mrow>
	</mdn>
	</p>
	
	<p>
	Let <m>n = p_1^{a_1} \dotsm p_k^{a_k}</m>.
	Then <m>r(n) = r(p_1^{a_1}) \dotsm r(p_k^{a_k})</m>.
	We saw that every <m>r(p^a) \geq 0</m>, hence <m>r(n) \geq 0</m>.
	If <m>n</m> is a perfect square, then every power <m>a_i</m> is even,
	so each <m>r(p_i^{a_i}) \geq 1</m>.
	It follows that <m>r(n) \geq 1</m>.
	</p>
	</proof>
	</claim>

	<claim>
	<title> Step 2 </title>
	<statement>
	<p>
	Let <m>A(x) = \sum_{n \leq x} \frac{r(n)}{\sqrt{n}}</m>.
	Then <m>A(x) \to \infty</m> as <m>x \to \infty</m>.
	</p>
	</statement>
	
	<proof>
	<p>
	We have
	<md>
	<mrow> A(x) \amp = \sum_{n \leq x} \frac{r(n)}{\sqrt{n}} </mrow>
	<mrow> \amp \geq \sum_{n \leq x, n = m^2} \frac{1}{\sqrt{n}} </mrow>
	<mrow> \amp = \sum_{m \leq \sqrt{x}} \frac{1}{m} </mrow>
	</md>
	This is a partial sum of the harmonic series; as <m>x \to \infty</m>
	it diverges.
	</p>
	</proof>
	
	</claim>
	
	<claim>
	<title> Step 3 </title>
	<statement>
	<p>
	<m>A(x) = 2\sqrt{x} L(1,\chi) + O(1) </m>.
	</p>
	</statement>
	
	<proof>
	<p>
	We will use the Dirichlet hyperbola method.
	</p>
	
	<p>
	We have
	<mdn>
	<mrow> A(x) \amp = \sum_{n \leq x} \frac{r(n)}{\sqrt{n}} </mrow>
	<mrow> \amp = \sum_{n \leq x} \frac{1}{\sqrt{n}} \sum_{d \mid n} \chi(d) </mrow>
	<mrow> \amp = \sum_{dk \leq x} \frac{\chi(d)}{\sqrt{dk}} </mrow>
	<mrow> \amp = \sum_{dk \leq x} \frac{\chi(d)}{\sqrt{d}} \cdot \frac{1}{\sqrt{k}} </mrow>
	</mdn>
	This sum is over lattice points <m>(d,k)</m> where <m>d,k</m> are postive
	integers such that <m>dk \leq x</m>, i.e., lying on or underneath the
	hyperbola <m>dk = x</m> in the <m>dk</m>-plane.
	We separate the region under the hyperbola into three parts as follows:
	the first part is defined by <m>d \leq \sqrt{x}</m>,
	the second is defined by <m>k \leq \sqrt{x}</m>,
	and the third is the intersection of the first two, so <m>d, k \leq \sqrt{x}</m> (both).
	Visually, if <m>d</m> is the horizontal coordinate and <m>k</m> is the vertical coordinate,
	then the region under the hyperbola with <m>d \leq \sqrt{x}</m> is the
	<lq/>upward<rq/> branch, the region under the hyperbola with <m>k \leq \sqrt{x}</m>
	is the <lq/>rightward<rq/> branch, and the region with both <m>d,k \leq \sqrt{x}</m>
	is a square.
	Define <m>S_1,S_2,S_3</m> as the sums over lattice points in these regions:
	<men>
		S_1 = \sum_{dk \leq x, d \leq \sqrt{x}} \frac{\chi(d)}{\sqrt{d}} \frac{1}{\sqrt{k}},
		\qquad
		S_2 = \sum_{dk \leq x, k \leq \sqrt{x}} \frac{\chi(d)}{\sqrt{d}} \frac{1}{\sqrt{k}},
		\qquad
		S_3 = \sum_{dk \leq x, d \leq \sqrt{x}, k \leq \sqrt{x}} \frac{\chi(d)}{\sqrt{d}} \frac{1}{\sqrt{k}}.
	</men>
	We have
	<men>
		A(x) = S_1 + S_2 - S_3.
	</men>
	</p>
	
	<p>
	Now our goal is to approximate the <m>S_i</m>.
	Looking ahead, we can expect to encounter certain sums,
	so it will be helpful to recall the following approximations:
	<men>
		\sum_{k \leq y} \frac{1}{k^s} = \frac{y^{-s+1}}{-s+1} + O(1)
	</men>
	and
	<men>
		\sum_{d \leq z} \frac{\chi(d)}{d^s} = L(s,\chi) + O\left(\frac{1}{z^s}\right)
	</men>,
	both of these holding for all <m>0 \lt s \lt 1</m>.
	(The textbook mentions a more accurate approximation for the sum of <m>1/k^s</m>
	that can be found by using Euler summation.)
	We will use them for <m>s = \frac{1}{2}</m>.
	In order to avoid headaches about fractions, here are explicit statements:
	<men>
		\sum_{k \leq y} \frac{1}{\sqrt{k}} = \frac{y^{1/2}}{1/2} + O(1) = 2\sqrt{y} + O(1)
	</men>
	and
	<men>
		\sum_{d \leq z} \frac{\chi(d)}{\sqrt{d}} = L(1/2,\chi) + O\left(\frac{1}{\sqrt{z}}\right)
	</men>.
	We will apply these with various <m>y</m>'s and <m>z</m>'s;
	warning, sometimes we will use, for example,
	<m>y = \sqrt{x}</m> in which case <m>\sqrt{y} = x^{1/4}</m> (similar for <m>z</m>).
	</p>
	
	<p>
	Now, here are the approximations of the <m>S_i</m>.
	The easiest is <m>S_3</m>:
	<mdn>
	<mrow> S_3 \amp = \left( \sum_{d \leq \sqrt{x}} \frac{\chi(d)}{\sqrt{d}} \right)
		\left( \sum_{k \leq \sqrt{x}} \frac{1}{\sqrt{k}} \right) </mrow>
	<mrow> \amp = (L(1/2,\chi) + O(1/x^{1/4})) (2x^{1/4} + O(1)) </mrow>
	<mrow> \amp = 2x^{1/4} L(1/2,\chi) + O(1) </mrow>
	</mdn>
	Next, we approximate <m>S_1</m>:
	<mdn>
	<mrow> S_1 \amp = \sum_{d \leq \sqrt{x}} \frac{\chi(d)}{\sqrt{d}} \sum_{k \leq \frac{x}{d}} \frac{1}{\sqrt{k}} </mrow>
	<mrow> \amp = \sum_{d \leq \sqrt{x}} \frac{\chi(d)}{\sqrt{d}} \left(2\sqrt{x/d} + O(1) \right) </mrow>
	<mrow> \amp = 2\sqrt{x} \sum_{d \leq \sqrt{x}} \frac{\chi(d)}{d} + O(1) \sum_{d \leq \sqrt{x}} \frac{\chi(d)}{\sqrt{d}} </mrow>
	<mrow> \amp = 2\sqrt{x} (L(1,\chi) + O(1/\sqrt{x})) + O(1)(L(1/2,\chi) + O(1/x^{1/4})) </mrow>
	<mrow> \amp = 2 \sqrt{x} L(1,\chi) + O(1) </mrow>
	</mdn>
	(For some reason, the textbook uses more accurate approximations here
	and does extra work, to arrive at the same result in the end.)
	Finally, <m>S_2</m> is similar to <m>S_1</m>:
	<mdn>
	<mrow> S_2 \amp = \sum_{k \leq \sqrt{x}} \frac{1}{\sqrt{k}} \sum_{d \leq \frac{x}{k}} \frac{\chi(d)}{\sqrt{d}} </mrow>
	<mrow> \amp = \sum_{k \leq \sqrt{x}} \frac{1}{\sqrt{k}} (L(1/2,\chi) + O(1/\sqrt{x/k})) </mrow>
	<mrow> \amp = L(1/2,\chi) \sum_{k \leq \sqrt{x}} \frac{1}{\sqrt{k}} + O(1/\sqrt{x}) \sum_{k \leq \sqrt{x}} \frac{1}{\sqrt{k}} O(\sqrt{k}) </mrow>
	<mrow> \amp = L(1/2,\chi) (2x^{1/4} + O(1)) + O(1/\sqrt{x}) O(\sqrt{x}) </mrow>
	<mrow> \amp = 2x^{1/4} L(1/2,\chi) + O(1) </mrow>
	</mdn>
	Putting it all together:
	<mdn>
	<mrow> A(x) \amp = S_1 + S_2 - S_3 </mrow>
	<mrow> \amp = (2 \sqrt{x} L(1,\chi) + O(1)) + (2 x^{1/4} L(1/2,\chi) + O(1)) - (2x^{1/4}L(1/2,\chi) + O(1)) </mrow>
	<mrow> \amp = 2 \sqrt{x} L(1,\chi) + O(1) </mrow>
	</mdn>
	which proves the claim.
	</p>
	</proof>
	
	</claim>
	
	<claim>
	<title> Conclusion </title>
	<statement><p><m>L(1,\chi) \neq 0</m>.</p></statement>
	
	<proof>
	<p>
	If <m>L(1,\chi)=0</m> then <m>A(x) = O(1)</m>,
	contradicting that <m>A(x) \to \infty</m> as <m>x \to \infty</m>.
	</p>
	</proof>
	</claim>
	
	</proof>
	

	</theorem>
  
  </subsection>
  
  <subsection>
  <title> Nonreal nonprincipal characters </title>
  
	<theorem>
	<statement>
	Let <m>\chi</m> be any nonprincipal Dirichlet character modulo <m>q</m>.
	Then <m>L(1,\chi) \neq 0</m>.
	</statement>
	
	<proof>
	<p>
	Let <m>N</m> be the number of Dirichlet characters <m>\chi</m> modulo <m>q</m>
	with <m>L(1,\chi) = 0</m>.
	Our goal is to show that <m>N = 0</m>.
	</p>
	
	<p>
	Recall that:
	<ol>
	<li> For the principal character <m>\chi_0</m>, <m>\sum_{n \leq x} \frac{\chi_0(n)\Lambda(n)}{n} = \log x + O(1)</m>. </li>
	<li> For <m>\chi \neq \chi_0</m>, if <m>L(1,\chi) \neq 0</m>, then <m>\sum_{n \leq x} \frac{\chi(n)\Lambda(n)}{n} = O(1)</m>. </li>
	<li> For <m>\chi \neq \chi_0</m>, if <m>L(1,\chi) = 0</m>, then <m>\sum_{n \leq x} \frac{\chi(n)\Lambda(n)}{n} = -\log x + O(1)</m>. </li>
	</ol>
	Adding this up for all characters modulo <m>q</m>, we get
	<men>
		\sum_{\chi \mod q} \sum_{n \leq x} \frac{\chi(n)\Lambda(n)}{n} = (1-N)\log x + O(1)
	</men>
	We get <m>+1\log x</m> from the principal character, and <m>-N\log x</m>
	from the nonprincipal characters with <m>L(1,\chi)=0</m>.
	</p>
	
	<p>
	We can use the orthogonality relations to simplify the left hand side of the equation:
	<mdn>
	<mrow> \sum_{\chi \mod q} \sum_{n \leq x} \frac{\chi(n)\Lambda(n)}{n}
		\amp = \sum_{n \leq x} \left( \sum_{\chi \mod q} \chi(n) \right) \frac{\Lambda(n)}{n} </mrow>
	<mrow> \amp = \phi(q) \sum_{n \leq x, n \equiv 1 \pmod{q}} \frac{\Lambda(n)}{n} </mrow>
	<mrow> \amp \geq 0 </mrow>
	</mdn>
	We used that <m>\sum_{\chi \mod q} \chi(n)</m> is equal to <m>\phi(q)</m>
	if <m>n \equiv 1 \pmod{q}</m>, or <m>0</m> otherwise.
	And we used that each term <m>\frac{\Lambda(n)}{n} \geq 0</m>.
	</p>
	
	<p>
	The result is that
	<me>
		(1-N)\log x + O(1) \geq 0
	</me>
	Well, if <m>N \gt 1</m> this is impossible, the left hand side will go to <m>-\infty</m>.
	Therefore <m>N \leq 1</m>.
	</p>
	
	<p>
	Finally we rule out the possibility that <m>N=1</m>.
	If <m>N=1</m> it means that there is a nonprincipal character <m>\chi</m>
	with <m>L(1,\chi) = 0</m>.
	We know that <m>\chi</m> must be nonreal, i.e., <m>\chi(a) \notin \bbR</m> for some <m>a</m>.
	</p>
	
	<p>
	But then <m>\overline{\chi}</m> is also a character, distinct from <m>\chi</m>
	(<m>\overline{\chi} \neq \chi</m>), and we have
	<me>
		L(1,\overline{\chi}) = \sum \frac{\overline{\chi}(n)}{n} = \overline{\sum \frac{\chi(n)}{n}}
		= \overline{L(1,\chi)} = 0
	</me>
	which would force <m>N \geq 2</m>.
	</p>
	
	<p>
	This contradiction shows that <m>N=1</m> is impossible.
	So it must be <m>N=0</m>.
	There are no Dirichlet characters <m>\chi</m> with <m>L(1,\chi)=0</m>.
	</p>
	</proof>	
	
	</theorem>

  </subsection>
  
  
  
  <subsection>
  <title> Conclusion: Proof of Dirichlet's theorem </title>
  
  <theorem>
  <title> Dirichlet's theorem </title>
  <statement>
  <p>
  Let <m>q,a</m> be positive integers with <m>(a,q)=1</m>.
  Then
  <me>
  	\sum_{p \leq x, p \equiv a \pmod{q}} \frac{\log p}{p} = \frac{1}{\phi(q)} \log x + O(1)
  </me>.
  In particular, there are infinitely many primes congruent to <m>a</m> modulo <m>q</m>.
  </p>
  </statement>
  
  <proof>
  <p>
  We have
  <mdn>
  <mrow> \sum_{p \leq x, p \equiv a \pmod{q}} \frac{\log p}{p}
  	\amp = \sum_{n \leq x, n \equiv a \pmod{q}} \frac{\Lambda(n)}{n} + O(1) </mrow>
  <mrow> \amp = \frac{1}{\phi(q)} \sum_{\chi \mod q} \overline{\chi}(a) \sum_{n \leq x} \frac{\chi(n)\Lambda(n)}{n} + O(1) </mrow>
  <mrow> \amp = \frac{1}{\phi(q)} \log x + \frac{1}{\phi(q)} \sum_{\chi \mod q, \chi \neq \chi_0} \sum_{n \leq x} \frac{\chi(n)\Lambda(n)}{n} + O(1) </mrow>
  <mrow> \amp = \frac{1}{\phi(q)} \log x + \frac{1}{\phi(q)} \sum_{\chi \mod q, \chi \neq \chi_0} O(1) + O(1) </mrow>
  <mrow> \amp = \frac{1}{\phi(q)} \log x + O(1) </mrow>
  </mdn>
  as claimed.
  </p>
  </proof>
  </theorem>
  
  
  
  </subsection>
  
</section>