<?xml version="1.0" encoding="UTF-8"?>

<section xml:id="sec-elementary-results" xmlns:xi="http://www.w3.org/2001/XInclude">
  <title>Elementary results on distribution of primes</title>
  
  <theorem>
  <statement>
  For <m>x \geq 5</m>, <m>\pi(x) \leq \theta(x)</m>.
  For <m>x \geq 1</m>, <m>\theta(x) \leq \psi(x)</m>.
  </statement>
  
  <proof>
  <p>
  We have <m>\pi(1) = 0</m>, <m>\pi(2) = 1</m>, <m>\pi(3) = 2</m>,
  <m>\pi(4) = 2</m>, and <m>\pi(5) = 3</m>.
  Meanwhile, <m>\theta(1) = 0</m>, <m>\theta(2) = \log 2</m>,
  <m>\theta(3) = \theta(4) = \log 2 + \log 3 \approx 1.79</m>,
  and <m>\theta(5) = \log 2 + \log 3 + \log 5 \approx 3.40</m>.
  So indeed <m>\theta(5) \geq \pi(5)</m>.
  For <m>p \geq 5</m> we have <m>\log p \gt 1</m>.
  So in the sums for <m>\theta</m> and <m>\pi</m>,
  all terms with <m>p \geq 5</m> are greater for <m>\theta</m>
  than for <m>\pi</m>.
  This shows that <m>\theta(x) \geq \pi(x)</m> for <m>x \geq 5</m>.
  </p>
  
  <p>
  The difference between <m>\theta</m> and <m>\psi</m> is
  <me>
    \psi(x) - \theta(x) = \sum_{p^k \leq x, k \geq 2} \log p
  </me>.
  This difference is always nonnegative because each
  <m>\log p \gt 0</m>.
  </p>
  </proof>
  </theorem>
  
  <theorem>
  <statement>
  For every <m>x \geq 1</m>, we have
  <men>
    0 \leq \psi(x) - \theta(x) \leq \frac{\sqrt{x}(\log x)^2}{2 \log 2}
  </men>.
  In particular, <m>\psi(x) = \theta(x) + O(\sqrt{x}(\log x)^2)</m>.
  </statement>
  
  <proof>
  <p>
  We already proved the first statement.
  For the second one,
  <md>
  <mrow> \psi(x) \amp = \sum_{n \leq x} \Lambda(n) </mrow>
  <mrow> \amp = \sum_{p^k \leq x} \log p </mrow>
  <mrow> \amp = \sum_{k=1}^{\infty} \sum_{p \leq x^{1/k}} \log p </mrow>
  <mrow> \amp = \sum_{k=1}^{\infty} \theta(x^{1/k}) </mrow>
  </md>.
  Despite appearances, this is actually a finite sum:
  We have <m>\theta(y) = 0</m> for <m>y \lt 2</m>.
  So <m>\theta(x^{1/k}) = 0</m> if <m>x^{1/k} \lt 2</m>,
  in other words if <m>k \gt \frac{\log x}{\log 2}</m>.
  Therefore
  <men>
    \psi(x) - \theta(x) = \sum_{2 \leq k \leq \frac{\log x}{\log 2}} \theta(x^{1/k})
  </men>.
  The largest term is <m>\theta(\sqrt{x})</m> (for <m>k=2</m>)
  and the number of terms is at most <m>\frac{\log x}{\log 2}</m>.
  Therefore the sum is bounded above,
  <me> \psi(x) - \theta(x) \leq \theta(\sqrt{x}) \frac{\log x}{\log 2} </me>.
  </p>
  
  <p>
  Furthermore,
  <men>
    \theta(\sqrt{x}) = \sum_{p \leq \sqrt{x}} \log p
    \leq \sum_{p \leq \sqrt{x}} \log \sqrt{x}
    \leq \sqrt{x} \log \sqrt{x}
  </men>
  since there are at at most <m>\sqrt{x}</m> terms.
  With this we get
  <men>
    \psi(x) - \theta(x) \leq \sqrt{x} (\log \sqrt{x}) \frac{\log x}{\log 2}
  </men>.
  After simplifying with <m>\log \sqrt{x} = \frac{1}{2} \log x</m>
  we have the claimed result.
  </p>
  </proof>
  </theorem>
  
  <remark>
  <p>
  Observe that twice in the above proof we bounded sums in the same way:
  bounding each term (every <m>\theta(x^{1/k})</m> is less than or equal to
  the largest one, which is <m>\theta(x^{1/2})</m>; every <m>\log p</m>
  is less than or equal to <m>\log \sqrt{x}</m>, when <m>p \leq \sqrt{x}</m>),
  and bounding the number of terms
  (in particular, a sum over primes <m>p \leq y</m> has at most <m>y</m> terms).
  </p>
  </remark>
  
  <p>
  The previous theorem gives a comparison between <m>\psi</m> and <m>\theta</m>.
  Now we give similar comparisons between <m>\theta</m> and the prime counting
  function <m>\pi</m>.
  </p>
  
  <theorem>
  <statement>
  For <m>x \geq 2</m> we have
  <men>
    \theta(x) = \pi(x) \log x - \int_2^x \frac{\pi(t)}{t} dt
  </men>
  and
  <men>
    \pi(x) = \frac{\theta(x)}{\log x} + \int_2^x \frac{\theta(t)}{t (\log t)^2} dt
  </men>.
  </statement>
  
  <proof>
  <p>
  The proof uses the Riemann-Stieltjes integral and integration by parts.
  Define a sequence by <m>a_n = 1</m> if <m>n</m> is a prime number
  and <m>a_n = 0</m> otherwise.
  Then <m>\pi(x) = \sum_{n \leq x} a_n</m>, and
  <mdn>
  <mrow xml:id="eqn-theta-pi-1"> \theta(x) \amp = \sum_{p \leq x} \log p </mrow>
  <mrow xml:id="eqn-theta-pi-2"> \amp = \sum_{1 \lt n \leq x} a_n \log n </mrow>
  <mrow xml:id="eqn-theta-pi-3"> \amp = \int_1^x \log t \; d\pi(t) </mrow>
  <mrow xml:id="eqn-theta-pi-4"> \amp = \pi(x) \log x - \int_1^x \frac{\pi(t)}{t} dt </mrow>
  <mrow xml:id="eqn-theta-pi-5"> \amp = \pi(x) \log x - \int_2^x \frac{\pi(t)}{t} dt </mrow>
  </mdn>.
  Here are the reasons for each step.
  <ul>
  <li><xref ref="eqn-theta-pi-1"/>: This is by the definition of <m>\theta</m></li>
  <li><xref ref="eqn-theta-pi-2"/>: This is by the definition of <m>a_n</m></li>
  <li><xref ref="eqn-theta-pi-3"/>: This the Riemann-Stieltjes integral</li>
  <li><xref ref="eqn-theta-pi-4"/>: Here we have used integration by parts</li>
  <li><xref ref="eqn-theta-pi-5"/>: For <m>x \lt 2</m>, <m>\pi(x) = 0</m></li>
  </ul>
  </p>
  
  <p>
  The second claim follows similarly.
  Let <m>b_n = \log n</m> if <m>n</m> is prime, <m>b_n = 0</m> otherwise.
  Then <m>\theta(x) = \sum_{n \leq x} b_n</m>, and
  <mdn>
  <mrow> \pi(x) \amp = \sum_{2 \leq n \leq x} \frac{1}{\log n} b_n </mrow>
  <mrow> \amp = \int_{2^{-}}^x \frac{1}{\log t} d\theta(t) </mrow>
  <mrow> \amp = \frac{\theta(x)}{\log x} + \int_2^x \frac{\theta(t)}{t (\log t)^2)} </mrow>
  </mdn>
  where we once again used the Riemann-Stelejes integral, and integration by parts.
  </p>
  </proof>
  </theorem>
  
  <p>
  One reason to care about the Chebyshev functions is that they give
  equivalent statements to the Prime Number Theorem:
  </p>
  <theorem>
  <statement>
  The following statements are equivalent:
  <ol>
  <li> <m>\pi(x) \sim \frac{x}{\log x}</m> </li>
  <li> <m>\theta(x) \sim x</m></li>
  <li> <m>\psi(x) \sim x</m></li>
  </ol>
  </statement>
  
  <proof>
  <p>
  We have
  <me>
    \theta(x) = \pi(x) \log x - \int_2^x \frac{\pi(t)}{t} dt,
  </me>.
  Dividing by <m>x</m> gives
  <me>
    \frac{\theta(x)}{x} = \frac{\pi(x)}{x/\log x} - \frac{1}{x} \int_2^x \frac{\pi(t)}{t} dt
  </me>.
  Assume that <m>\pi(x) \sim x/\log x</m>.
  We need to show that the integral term goes to zero.
  In this case we have <m>\frac{\pi(t)}{t} \ll \frac{1}{\log t}</m>.
  Therefore
  <me>
    \int_2^x \frac{\pi(t)}{t} dt \ll \int_2^x \frac{1}{\log t} dt
  </me>,
  because there is a threshold <m>T</m> and constant <m>C</m>
  such that for <m>t \gt T</m>, <m>\frac{\pi(t)}{t} \leq C \frac{1}{\log t}</m>;
  then for <m>x \gt T</m>,
  <me>
    \int_T^x \frac{\pi(t)}{t} dt \ll C \int_T^x \frac{1}{\log t} dt
  </me>.
  Notice that these integrals diverge to infinity as <m>x \to \infty</m>.
  The error (difference) between <m>\int_2^T \frac{\pi(t)}{t} dt</m>
  and <m>C \int_2^T \frac{1}{\log t} dt</m> is some constant amount;
  eventually it is insignificant compared to the integrals from <m>T</m> to <m>x</m>,
  for large <m>x</m> (and we can replace <m>C</m> with, say, <m>2C</m>).
  </p>
  
  <p>
  So, we have:
  <me>
    \frac{1}{x} \int_2^x \frac{\pi(t)}{t} dt \ll \frac{1}{x} \int_2^x \frac{1}{\log t} dt
  </me>
  We can bound the last integral in a similar way to previous bounds 
  of sums:
  the maximum value of the integrand on this interval is <m>\frac{1}{\log 2}</m>
  (because the function <m>\frac{1}{\log t}</m> is monotone decreasing)
  and the length of the interval is less than <m>x</m>.
  So the value of the integral is less than or equal to <m>\frac{x}{\log 2}</m>.
  This gives us:
  <md>
  <mrow> \frac{1}{x} \int_2^x \frac{\pi(t)}{t} dt \amp \ll \frac{1}{x} \int_2^x \frac{1}{\log t} dt </mrow>
  <mrow> \amp \ll \frac{1}{x} \frac{x}{\log 2} </mrow>
  <mrow> \amp = \frac{1}{\log 2} </mrow>
  </md>.
  So the <lq/>error<rq/> term (the integral) is bounded by a constant.
  But we want a stronger result: we want the error to go to zero.
  </p>
  
  <p>
  We can get this by a trick that is slightly reminiscent of the
  hyperbola method: we split the interval of integration
  into two parts as follows.
  <md>
  <mrow> \frac{1}{x} \int_2^x \frac{\pi(t)}{t} dt \amp \ll \frac{1}{x} \int_2^x \frac{1}{\log t} dt </mrow>
  <mrow> \amp = \frac{1}{x} \int_2^{\sqrt{x}} \frac{1}{\log t} dt + \frac{1}{x} \int_{\sqrt{x}}^x \frac{1}{\log t} dt </mrow>
  <mrow> \amp \ll \frac{1}{x} \frac{\sqrt{x}}{\log 2} + \frac{1}{x} \frac{x}{\log \sqrt{x}} </mrow>
  <mrow> \amp = \frac{1}{\sqrt{x} \log 2} + \frac{1}{\log \sqrt{x}} </mrow>
  </md>.
  This does go to zero.
  Therefore, if <m>\frac{\pi(x)}{x/\log x} \to 1</m>, then <m>\frac{\theta(x)}{x} \to 1</m> as well.
  </p>
  
  <remark>
  <p>
  By splitting the interval of integration into two parts,
  we have one part where the bound for the integrand is the same (<m>1/\log 2</m>)
  but the interval is shorter (<m>\sqrt{x}</m> instead of <m>x</m>)
  and another part where the interval is the same length
  (or rather, we use the same bound <m>x</m> for its length)
  but the integrand is bounded by a smaller amount
  (<m>1/\log \sqrt{x}</m> instead of <m>1/\log 2</m>).
  </p>
  </remark>
  
  <p>
  The converse (<m>\frac{\theta(x)}{x} \to 1</m> implies <m>\frac{\pi(x)}{x/\log x} \to 1</m>)
  is similar.
  </p>
  
  <p>
  From our comparison of <m>\psi</m> and <m>\theta</m> we have
  <me>
    0 \leq \frac{\psi(x)}{x} - \frac{\theta(x)}{x} \leq \frac{(\log x)^2}{2 \log 2 \sqrt{x}}
  </me>.
  Therefore
  <me>
    \lim_{x \to \infty} \frac{\psi(x)}{x} - \frac{\theta(x)}{x} = 0
  </me>,
  so
  <me>
    \frac{\psi(x)}{x} \to 1 \Leftrightarrow \frac{\theta(x)}{x} \to 1
  </me>.
  </p>
  </proof>
  </theorem>

  

</section>