<?xml version="1.0" encoding="UTF-8"?>

<section xml:id="sec-elementary-properties" xmlns:xi="http://www.w3.org/2001/XInclude">
  <title>Elementary properties of the floor function</title>
  
  <p>
  The floor function has many elementary properties listed in the textbook.
  Here are a few.
  </p>

	<proposition>
	<statement>
	For any real numbers <m>x</m> and <m>y</m>, and integer <m>n</m>:
	<ol>
	<li> <m>\lfloor n + x \rfloor = n + \lfloor x \rfloor </m> </li>
	<li> <m>\lfloor x \rfloor + \lfloor y \rfloor
		\leq \lfloor x + y \rfloor \leq \lfloor x \rfloor + \lfloor y \rfloor + 1 </m> </li>
	<li> <m>\lfloor -x \rfloor = - \lceil x \rceil </m> </li>
	</ol>
	</statement>
	
	<proof>
	<p>
	For the first statement, <m>n + \lfloor x \rfloor</m> is an integer
	which is less than or equal to <m>n + x</m>.
	Since <m>\lfloor n + x \rfloor</m> is defined as the greatest integer
	less than or equal to <m>n + x</m>, it must be that this integer
	<m>n + \lfloor x \rfloor</m> is less than or equal to the greatest integer,
	so <m>n + \lfloor x \rfloor \leq \lfloor n + x \rfloor</m>.
	</p>

	<p>
	On the other hand, <m>\lfloor n + x \rfloor - n</m> is an integer
	which is less than or equal to <m>(n+x)-n = x</m>.
	Therefore <m>\lfloor n + x \rfloor - n \leq \lfloor x \rfloor</m>.
	This shows that <m>lfloor n + x \rfloor \leq n + \lfloor x \rfloor </m>.
	</p>

	<p>
	For the second statement,
	observe that <m>\lfloor x \rfloor + \lfloor y \rfloor</m> is an integer
	which is less than or equal to <m>x + y</m>.
	Therefore it is less than or equal to <m>\lfloor x + y \rfloor</m>.
	</p>
	
	<p>
	As before, <m>\lfloor x + y \rfloor - \lfloor x \rfloor</m>
	is an integer which is less than or equal to <m>x + y - \lfloor x \rfloor</m>.
	We have <m>x - \lfloor x \rfloor \leq 1</m> (in fact, strictly less)
	(because if <m>x - \lfloor x \rfloor \geq 1</m> then <m>\lfloor x \rfloor + 1 \leq x</m>,
	contradicting the maximality of <m>\lfloor x \rfloor</m>).
	Putting it together we have
	<me>
		\lfloor x + y \rfloor - \lfloor x \rfloor \leq x + y - \lfloor x \rfloor
			\leq y + 1
	</me>.
	Therefore
	<me>
		\lfloor x + y \rfloor - \lfloor x \rfloor \leq \lfloor y+1 \rfloor = \lfloor y + \rfloor + 1
	</me>.
	</p>
	
	<p>
	Finally, to see that <m>\lfloor -x \rfloor = - \lceil x \rceil</m>,
	observe that <m>m \leq -x</m> if and only if <m>-m \geq x</m>.
	</p>

	
	</proof>

	</proposition>


		


</section>