<?xml version="1.0" encoding="UTF-8"?>

<section xml:id="sec-hermite-identity" xmlns:xi="http://www.w3.org/2001/XInclude">
  <title>Hermite's Identity</title>
  
  <theorem>
  <title>Hermite's Identity</title>
  <statement>
  For any real <m>x</m> and positive integer <m>n</m>,
  <men>
  	\sum_{0 \leq k \leq n-1} \left\lfloor x + \frac{k}{n} \right\rfloor
  	= \lfloor n x \rfloor
  </men>
	</statement>
	</theorem>

	<example>
	If <m>n=1</m> the statement says:
	<me>
		\sum_{k=0} \left\lfloor x + \frac{k}{1} \right\rfloor
		= \lfloor x + 0 \rfloor
		= \lfloor 1 x \rfloor
	</me>.
	If <m>n=2</m> the statement says:
	<me>
		\sum_{0 \leq k \leq 1} \left\lfloor x + \frac{k}{n} \right\rfloor
		= \lfloor x \rfloor + \left\lfloor x + \frac{1}{2} \right\rfloor
	</me>.
	Say <m>\lfloor x \rfloor = m</m>.
	If <m>m \leq x \lt m + \frac{1}{2}</m> then
	<me>
		\lfloor x \rfloor + \left\lfloor x + \frac{1}{2} \right\rfloor
		= m + m = 2m
	</me>
	and
	<me> \lfloor 2x \rfloor = 2m </me>
	because <m>2m \leq 2x \lt 2m+1</m>.
	Otherwise if <m>m + \frac{1}{2} \leq x \lt m+1</m> then
	<me>
		\lfloor x \rfloor + \left\lfloor x + \frac{1}{2} \right\rfloor
		= m + (m+1) = 2m+1 = \lfloor 2x \rfloor
	</me>
	because <m>2m+1 \leq 2x \lt 2m+2</m>.
	</example>
	
	
	<p>
	The textbook gives several generalizations of this theorem,
	for example summing <m>0 \leq k \leq m-1</m> where <m>m</m>
	can be a different integer than <m>n</m>.
	For class we'll just give a direct proof of Hermite's identity
	rather than one of the generalizations.
	</p>

	
	<proof>
	<p>
	Let <m>m</m> be the integer such that
	<me> \frac{m}{n} \leq x \lt \frac{m+1}{n} </me>,
	in other words <m> m = \lfloor n x \rfloor</m>.
	Write <m>m = q n + r</m> where <m>0 \leq r \lt n</m>.
	Observe that <m>q + \frac{r}{n} \leq x \lt q + \frac{r+1}{n}</m>.
	In particular <m>\lfloor x \rfloor = q</m>.
	</p>
	
	<p>
	For <m>0 \leq k \leq n - r - 1</m> we have
	<md>
	<mrow> q \amp \leq x </mrow>
	<mrow> \amp \leq x + \frac{k}{n} </mrow>
	<mrow> \amp \lt \frac{m+1}{n} + \frac{k}{n} </mrow>
	<mrow> \amp \leq \frac{q n + r + 1 + (n-r-1)}{n} </mrow>
	<mrow> \amp = q + 1 </mrow>
	</md>.
	That is,
	<me> q \leq x + \frac{k}{n} \lt q+1 </me>.
	Then <m> \left\lfloor x + \frac{k}{n} \right\rfloor = q </m>.
	</p>
	
	<p>
	For <m>n-r \leq k \leq n-1</m> we have
	<md>
	<mrow> q+1 \amp = q + \frac{r}{n} + \frac{n-r}{n} </mrow>
	<mrow> \amp \leq x + \frac{k}{n} </mrow>
	<mrow> \amp \lt \frac{m+1}{n} + \frac{k}{n} </mrow>
	<mrow> \amp \leq \frac{q n + r + n-1}{n} </mrow>
	<mrow> \amp \leq \frac{q n + n + n}{n} </mrow>
	<mrow> \amp = q + 2 </mrow>
	</md>.
	So <m>q+1 \leq x + \frac{k}{n} \lt q+2</m>.
	Therefore <m>\left\lfloor x + \frac{k}{n} \right\rfloor = q+1</m>.
	</p>

  <p>
  Now the sum in Hermite's identity has <m>n-r</m> terms
  that are equal to <m>q</m>, and <m>r</m> terms that are
  equal to <m>q+1</m>.
  So the sum is equal to <m>(n-r)q + r(q+1)</m>,
  which is equal to <m>nq+r = m = \lfloor n x \rfloor</m>.
  </p>

	
	</proof>


	


</section>