<?xml version="1.0" encoding="UTF-8"?>

<section xml:id="sec-average-order" xmlns:xi="http://www.w3.org/2001/XInclude">
  <title>Average Order of Growth</title>
  
  <introduction>
	<p>
	Recall some of the previously defined arithmetic functions:
	<ol>
	<li><m>d(n)</m>: number of positive divisors of <m>n</m></li>
	<li><m>\sigma(n)</m>: sum of positive divisors of <m>n</m></li>
	</ol>
	These can <lq/>oscillate<rq/> wildly:
	for example <m>d(n)</m> can be arbitrarily large (<m>d(2^{k-1}) = k</m>)
	and it also drops down to <m>d(n)=2</m> infinitely often (specifically, at primes).
	We can <lq/>smooth out the oscillations<rq/> by averaging.
	That is, for any <m>x \gt 1</m>, we consider
	the average value of <m>d(n)</m> for all <m>n</m> up to <m>x</m>:
	<me> \frac{1}{x} \sum_{n \leq x} d(n) </me>.
	Similarly for <m>\sigma</m> and any other arithmetic function.
	</p>
	
	<p>
	The book uses capital letters for averages.
	Thus if <m>f</m> is an arithmetic function, then
	<m>F</m> is the average,
	<me> F(x) = \frac{1}{x} \sum_{n \leq x} f(n) </me>.
	Unless confusion seems likely, it may be preferable to use an overline,
	as in <m>\overline{f}</m>:
	<me> \overline{f}(x) = \frac{1}{x} \sum_{n \leq x} f(n) </me>.
	</p>
	
	<p>
	Observe that the domain of the average function is the real numbers
	rather than the positive integers.
	At this point, this is a more or less arbitrary choice (<lq/>why not<rq/>).
	</p>
	
	<definition>
	<p>
	Let <m>f</m> be an arithmetic function.
	We say <m>g</m> is an <term>average order</term> of <m>f</m>
	if <m>g</m> is positive and
	<men> \overline{f}(x) \sim \frac{1}{x} \sum_{n \leq x} g(n) </men>.
	Typically we require <m>g</m> to be monotone.
	</p>
	</definition>
	
	<p>
	The average order is not unique.
	For example, if <m>g</m> is an average order for <m>f</m>
	and <m>g'(n) = g(n)</m> for all but finitely many <m>n</m>,
	then <m>g'</m> is also an average order for <m>f</m>.
	Indeed, the difference between summing <m>g(n)</m> and summing <m>g'(n)</m>
	is some constant (finite) value; after dividing by <m>x</m>,
	the difference goes to zero as <m>x \to \infty</m>.
	</p>
	
	<p>
	Nevertheless we will say <lq/>the average order<rq/>
	instead of <lq/>an average order<rq/>, just because it sounds nicer.
	</p>
	
	
	</introduction>
	
	<subsection>
	<title>Average order of number of divisors</title>
	
	<theorem>
	<statement>
	For <m>d(n)</m>, the number of positive divisors of <m>n</m>,
	we have <m>\sum_{n \leq x} d(n) = x \log x + O(x)</m>.
	Thus, <m>\overline{d}(x) \sim \log x</m>.
	The average order of <m>d(n)</m>, the number of divisors of <m>n</m>,
	is <m>\log n</m>.
	That is,
	<m>\overline{d}(x) = \frac{1}{x}\sum_{n \leq x} d(n) \sim \frac{1}{x} \sum_{n \leq x} \log n</m>.
  </statement>
  
  <proof>
  <p>
  We have
  <md>
  <mrow> \sum_{n \leq x} d(n) \amp = \sum_{n \leq x} \sum_{d \mid n} 1 </mrow>
  <mrow> \amp = \sum_{d \leq x} \sum_{n \leq x, d \mid n} 1 </mrow>
  <mrow> \amp = \sum_{d \leq x} \sum_{dk \leq x} 1 </mrow>
  <mrow> \amp = \sum_{d \leq x} \left\lfloor \frac{x}{d} \right\rfloor </mrow>
  <mrow> \amp = \sum_{d \leq x} \left( \frac{x}{d} + O(1) \right) </mrow>
  <mrow> \amp = x \sum_{d \leq x} \frac{1}{d} + O(x) </mrow>
  <mrow> \amp = x (\log x + O(1)) + O(x) </mrow>
  <mrow> \amp = x \log x + O(x) </mrow>
  </md>.
  We used <m>\sum_{d \leq x} \frac{1}{d} = \log x + O(1)</m>.
  </p>
  
  <p>
  From this it follows that
  <me>
    \overline{d}(x) = \frac{1}{x} \sum_{n \leq x} d(n) = \log x + O(1)
  </me>.
  In particular
  <me>
    \frac{\overline{d}(x)}{\log x} = 1 + \frac{O(1)}{\log x}
  </me>.
  The fraction on the right goes to zero as <m>x \to \infty</m>,
  hence <m>\overline{d}(x) \sim \log x</m> as claimed.
  </p>
  
  <p>
  Finally, we have seen that
  <me> \sum_{n \leq x} \log n = x \log x - x + O(1) </me>.
  After dividing by <m>x</m> we get <m>\log x + O(1)</m>,
  matching <m>\overline{d}(x)</m>.
  </p>
  </proof>
  </theorem>
  
	</subsection>
	
	<subsection>
	<title>Average order of sum of divisors</title>
	
	<theorem>
	<statement>
	For the divisor sum function <m>\sigma</m> we have
	<m>\sum_{n \leq x} \sigma(n) = \frac{\pi^2}{12} x^2 + O(x \log x)</m>.
	</statement>
	
	<proof>
	<p>
	We have
	<md>
	<mrow> \sum_{n \leq x} \sigma(n) \amp = \sum_{n \leq x} \sum_{d \mid n} d </mrow>
	<mrow> \amp = \sum_{dk \leq x} d </mrow>
	<mrow> \amp = \sum_{k \leq x} \sum_{d \leq x/k} d </mrow>
	<mrow> \amp = \sum_{k \leq x} \frac{1}{2} \left\lfloor \frac{x}{k} \right\rfloor \left( \left\lfloor \frac{x}{k} \right\rfloor + 1 \right) </mrow>
	<mrow> \amp = \frac{1}{2} \sum_{k \leq x} \left( \frac{x^2}{k^2} + O(x/k) \right) </mrow>
	<mrow> \amp = \frac{1}{2} x^2 \sum_{k \leq x} \frac{1}{k^2} + O\left( x \sum_{k \leq x} \frac{1}{k} \right) </mrow>
  </md>.
  We can use
  <me> \sum_{k \leq x} \frac{1}{k} = \log x + O(1) </me>
  to rewrite
  <me> O\left( x \sum_{k \leq x} \frac{1}{k} \right) = O(x \log x) + O(x) = O(x \log x) </me>.
  </p>
  
  <p>
  For the <m>x^2</m> term, we use these facts.
  First,
  <men> \sum_{k = 1}^\infty \frac{1}{k^2} = \frac{\pi^2}{6} </men>.
  This is Euler's solution of the Basel problem.
  For now we will use this without giving a proof
  (many proofs exist and can be found in various textbooks or online).
  Second, we have seen that for <m>\alpha \gt 1</m>,
  <men> \sum_{n \gt x} \frac{1}{n^\alpha} = O(x^{-\alpha+1}) </men>.
  Combining these,
  <md>
  <mrow> \frac{1}{2} x^2 \sum_{k \leq x} \frac{1}{k^2}
    \amp = \frac{1}{2} x^2 \left( \sum_{k=1}^\infty \frac{1}{k^2} - \sum_{k \gt x} \frac{1}{k^2} \right) </mrow>
  <mrow> \amp = \frac{1}{2} x^2 \left( \frac{\pi^2}{6} - O(x^{-1}) \right) </mrow>
  <mrow> \amp = \frac{\pi^2}{12} x^2 - O(x) </mrow>
  </md>.
  This completes the proof.
  </p>
  </proof>
  </theorem>
  
  <corollary>
  <statement>
  The average order of <m>\sigma(n)</m> is <m>\frac{\pi^2}{6} n</m>.
  </statement>
  
  <proof>
  <p>
  The claim is that
  <me> \frac{1}{x} \sum_{n \leq x} \sigma(n) \sim \frac{1}{x} \sum_{n \leq x} \frac{\pi^2}{6} n </me>.
  The left hand side is
  <me> \frac{1}{x} \sum_{n \leq x} \sigma(n) = \frac{\pi^2}{12} x + O(\log x) </me>
  and the right hand side is
  <md>
  <mrow> \frac{1}{x} \sum_{n \leq x} \frac{\pi^2}{6} n \amp = \frac{\pi^2}{12} \frac{1}{x} \lfloor x \rfloor ( \lfloor x \rfloor + 1 ) </mrow>
  <mrow> \amp = \frac{\pi^2}{12} x + O(1) </mrow>
  </md>.
  The two quantities are asymptotic since
  <me>
    \lim_{x \to \infty} \frac{\frac{\pi^2}{12} x + O(\log x)}{\frac{\pi^2}{12} x + O(1) } = 1
  </me>.
  </p>
  </proof>
  </corollary>
  
  <p>
  This is not quite the same thing as saying that the average value of
  <m>\sigma(n)/n</m> should be <m>\pi^2/6</m>.
  In our statements above we averaged <m>\sigma(n)</m>.
  We have not evaluated the sum or the average of <m>\sigma(n)/n</m>.
  </p>
  
  <proposition>
  <statement>
  <men> \sum_{n \leq x} \frac{\sigma(n)}{n} = \frac{\pi^2}{6} x + O(\log x) </men>.
  </statement>
  
  <proof>
  <p>
  We have
  <md>
  <mrow> \sum_{n \leq x} \frac{\sigma(n)}{n} \amp = \sum_{n \leq x} \frac{1}{n} \sum_{d \mid n} d </mrow>
  <mrow> \amp = \sum_{dk \leq x} \frac{d}{dk} </mrow>
  <mrow> \amp = \sum_{dk \leq x} \frac{1}{k} </mrow>
  <mrow> \amp = \sum_{k \leq x} \sum_{d \leq x/k} \frac{1}{k} </mrow>
  <mrow> \amp = \sum_{k \leq x} \frac{1}{k} \left\lfloor \frac{x}{k} \right\rfloor </mrow>
  <mrow> \amp = \sum_{k \leq x} \frac{1}{k} \left( \frac{x}{k} - \left\{ \frac{x}{k} \right\} \right) </mrow>
  <mrow> \amp = \sum_{k \leq x} \frac{x}{k^2} - O(\sum_{k \leq x} \frac{1}{k}) </mrow>
  <mrow> \amp = \frac{\pi^2}{6} x - O(1/x) - O(\log x) </mrow>
  </md>.
  This completes the proof.
  </p>
  </proof>
  </proposition>
  
  </subsection>
  
  <subsection>
  <title>Average order of Euler totient</title>
  
  <theorem>
  <statement>
  <m>\sum_{n \leq x} \varphi(n) = \frac{3}{\pi^2} x^2 + O(x \log x) </m>.
  </statement>
  
  <proof>
  <p>
  The proof is similar to before.
  We use
  <me> \varphi(n) = n \sum_{d \mid n} \frac{\mu(d)}{d} </me>,
  where <m>\mu</m> is the MÃ¶bius function.
  After some algebra very similar to the proof of the previous theorem,
  <me>
    \sum_{n \leq x} \varphi(n) = \frac{1}{2} x^2 \left( \sum_{d=1}^\infty \frac{\mu(d)}{d^2} \right) + O(x \log x)
  </me>.
  We have mentioned that
  <men>
    \left(\sum_{n=1}^\infty \frac{1}{n^s} \right) \left(\sum_{n=1}^\infty \frac{\mu(n)}{n^s} \right) = 1
  </men>,
  so in particular for <m>s=2</m> we get
  <men>
    \sum_{n=1}^{\infty} \frac{\mu(n)}{n^2} = \frac{1}{\sum_{n=1}^{\infty} \frac{1}{n^2}}
    = \frac{1}{\pi^2/6} = \frac{6}{\pi^2}
  </men>.
  This completes the proof.
  </p>
  </proof>
  </theorem>
  
  </subsection>
  
  

</section>