<?xml version="1.0" encoding="UTF-8"?>

<section xml:id="sec-euler-summation" xmlns:xi="http://www.w3.org/2001/XInclude">
  <title>Euler Summation</title>
  
  <theorem>
  <title>Euler's summation formula</title>
  <statement>
  Let <m>0 \lt y \lt x</m> be real numbers and assume that
  <m>f : [y,x] \to \bbR</m> has a continuous derivative on <m>[y,x]</m>.
  Then
  <men>
    \sum_{y \lt n \leq x} f(n)
    = \int_y^x f(t) dt + \int_y^x \{t\} f'(t) dt
    + \{y\}f(y) - \{x\}f(x)
  </men>
  (where <m>\{t\}</m> denotes the fractional part of <m>t</m>,
  and similarly for <m>\{x\},\{y\}</m>).
  </statement>
  
  <proof>
  Observe that <m>\lfloor t \rfloor</m> is a step function with jump <m>1</m>
  at each integer, so
  <men>
    \sum_{y \lt n \leq x} f(n) = \int_y^x f d\lfloor t \rfloor
  </men>.
  We apply linearity of the Riemann-Stieltjes integral
  with respect to <m>t = \lfloor t \rfloor + \{t\}</m>,
  so that <m>dt = d\lfloor t \rfloor + d\{t\}</m>.
  This gives
  <men>
    \sum_{y \lt n \leq x} f(n) = \int_y^x f dt - \int_y^x f d\{t\}
  </men>.
  By integration by parts,
  <men>
    \int_y^x f d\{t\} = \left. f(t)\{t\} \right|_y^x - \int_y^x \{t\} f'(t) dt
  </men>
  and the result follows.
  </proof>
  </theorem>

</section>