<?xml version="1.0" encoding="UTF-8"?>

<section xml:id="sec-af1-mobius-inversion" xmlns:xi="http://www.w3.org/2001/XInclude">
  <title>Möbius inversion</title>
  
  <subsection>
  <title>Möbius function</title>
  
  <theorem>
  <statement>
  The following arithmetic functions are all equal:
  <ol>
  <li><m>\mu_1</m> defined in terms of factorization:
  	<men> \mu_1(n) = \begin{cases}
  		1 \amp \text{if } n = 1 \\
  		(-1)^k \amp \text{if } n = p_1 p_2 \dotsm p_k \\
  		0 \amp \text{if some } p^2 \mid n
  		\end{cases}
		</men>
	</li>
	<li><m>\mu_2</m> defined in terms of coefficients of a product:
		For any <m>n</m> we define <m>\mu_2</m> by
		<men> \prod_{p \mid n} \left( 1 - \frac{1}{p^s} \right) = \sum_{d \mid n} \frac{\mu_2(d)}{d^s} </men>.
		Here the product is over all primes <m>p</m> that divide <m>n</m>,
		while the sum is over all (positive) divisors of <m>n</m>.
		The symbol <m>s</m> is a formal variable; alternatively we can interpret
		this as saying that the two sides of the equation are equal for all
		complex numbers <m>s</m>.
		(We follow normal exponent rules, <m>1^s = 1</m> and <m>a^s b^s = (ab)^s</m>.)
		We assert that this function <m>\mu_2</m> is well-defined in the sense
		that if <m>d \mid n</m> and <m>d \mid n'</m>, then <m>\frac{1}{d^s}</m> has
		the same coefficient whether the product is taken over the primes that
		divide <m>n</m>, or primes that divide <m>n'</m>.
		In fact <m>\mu_2(d)</m> is the coefficient of <m>\frac{1}{d^s}</m>
		in the infinite product <m>\prod_p \left( 1 - \frac{1}{p^s} \right)</m>
		over all primes (this is a formal product in the sense that we don't worry
		about whether it converges).
	</li>
	<li><m>\mu_3</m> defined recursively: We define <m>\mu_3(1) = 1</m>
		and for <m>n \gt 1</m>, we define <m>\mu_3(n)</m> by setting
		<m>\sum_{d \mid n} \mu_3(d) = 0</m>.
	</li>
	<li><m>\mu_4</m> defined as the Dirichlet inverse of the arithmetic function
		<m>1(n) = 1</m> for all <m>n</m>.
	</li>
	</ol>
	That is, for all <m>n</m>, <m>\mu_1(n) = \mu_2(n) = \mu_3(n) = \mu_4(n)</m>.
	</statement>
	</theorem>

	<example>
	<p>
	For example,
	<men>
		\prod_{p \mid 6} \left( 1 - \frac{1}{p^s} \right)
		= \left( 1 - \frac{1}{2^s} \right) \left( 1 - \frac{1}{3^s} \right)
		= 1 - \frac{1}{2^s} - \frac{1}{3^s} + \frac{1}{6^s}
	</men>.
	This shows that <m>\mu_2(1) = 1</m>, <m>\mu_2(2) = -1</m>,
	<m>\mu_2(3) = -1</m>, and <m>\mu_2(6) = 1</m>.
	</p>
	
	<p>
	Likewise,
	<men>
		\prod_{p \mid 4} \left( 1 - \frac{1}{p^s} \right)
		= 1 - \frac{1}{2^s}
		= 1 - \frac{1}{2^s} + \frac{0}{4^s}
	</men>.
	This gives <m>\mu_2(2) = -1</m>, agreeing with the result when the product
	was taken over primes <m>p \mid 6</m> instead of <m>p \mid 4</m>.
	In addition we see that <m>\mu_2(4) = 0</m>.
	</p>

	</example>
	
	<proof>
	<p>
	The recursive definition of <m>\mu_3</m> means precisely that
	<m>\mu_3 * 1 = e</m>.
	Therefore <m>\mu_3</m> is the Dirichlet inverse of <m>1</m>,
	so <m>\mu_3 = \mu_4</m>.
	(Note: Dirichlet inverses are unique: if <m>f * g_1 = f * g_2 = e</m>,
	then <m>g_1 = g_2</m> (why?).)
	</p>
	
	<p>
	Suppose <m>d \mid n</m>, <m>d \gt 1</m>,
	and <m>d = p_1^{a_1} \dotsm p_k^{a_k}</m>
	where the <m>p_i</m> are distinct primes and each <m>a_i \geq 1</m>.
	First, each <m>p_i</m> divides <m>n</m> as well,
	so the product in the definition of <m>\mu_2</m> includes all of the primes
	<m>p_i</m> appearing in the prime factorization of <m>d</m>.
	If any <m>p_i^2 \mid d</m> then <m>\mu_2(d) = 0</m>,
	since the product only includes one factor of <m>1/p_i^s</m>;
	there is no <m>1/(p_i^2)^s</m>.
	(Here is where the formal variable <m>s</m> plays a role:
	without it, we could have <m>1/p_i = p_i / p_i^2</m>,
	and the sum could be rewritten to include a term with denominator <m>p_i^s</m>.
	With the <m>s</m> however, we have <m>1/p_i^s = p_i^s / (p_i^2)^s</m>,
	and we are requiring that the numerators only involve <m>\mu_2(d)</m>'s,
	without any <m>s</m>.)
	Otherwise, if each <m>a_i = 1</m>, so <m>d = p_1 p_2 \dotsm p_k</m>,
	then
	<men> \frac{\mu_2(d)}{d^s} = \frac{-1}{p_1^s} \frac{-1}{p_2^s} \dotsm \frac{-1}{p_k^s}
		= \frac{(-1)^k}{(p_1 \dotsm p_k)^s} </men>.
	This shows that in this case <m>\mu_2(d) = (-1)^k</m>.
	Finally for <m>d = 1</m> we have <m>\mu_2(1) = 1</m>
	because the term of the product with denominator <m>1^s = 1</m>
	is given by multiplying <m>1</m> for each prime <m>p \mid n</m>.
	</p>
	
	<p>
	This shows that <m>\mu_2(d) = \mu_1(d)</m> for all <m>d \mid n</m>.
	In particular, <m>\mu_2(d)</m> doesn't actually depend on which multiple
	<m>n</m> of <m>d</m> is used.
	Therefore <m>\mu_2 = \mu_1</m>.
	The fact that we can take the infinite product follows from the observation
	that including factors <m>1 - \frac{1}{p^s}</m> where <m>p \gt d</m>
	has no effect on the coefficient of <m>\frac{1}{d^s}</m>.
	</p>

	<p>
  Finally we prove that <m>\mu_1 * 1 = e</m>, which gives <m>\mu_1 = \mu_4</m>.
  We have <m>(\mu_1 * 1)(1) = \mu_1(1) 1(1) = 1 = e(1)</m> by definition.
  For <m>n \gt 1</m>, say <m>n = p_1^{a_1} \dotsm p_k^{a_k}</m>
  where the <m>p_i</m> are distinct primes and each <m>a_i \geq 1</m>.
  Let <m>d \mid n</m> and write <m>d = p_1^{b_1} \dotsb p_k^{b_k}</m>.
  By definition of <m>\mu_1</m>, if any <m>b_i \gt 1</m>
  then <m>\mu_1(d) = 0</m>.
  So in the sum <m>(\mu_1 * 1)(n) = \sum_{d \mid n} \mu_1(d)</m>
  we can ignore such terms, and only include terms <m>d \mid n</m>
  such that in the prime factorization, every prime appears with
  power <m>0</m> or <m>1</m>.
	</p>
	
	<p>
	Let <m>[k] = \{1,\dotsc,k\}</m>.
	For a subset <m>S \subseteq [k]</m> let <m>d_S = \prod_{i \in S} p_i</m>,
	that is, <m>d_S</m>is the product of primes in the prime factorization
	of <m>n</m> corresponding to elements of <m>n</m>.
	In particular if <m>S = \varnothing</m> then <m>d_{\varnothing} = 1</m>.
	By the definition of <m>\mu_1</m>, <m>\mu_1(d_S) = (-1)^{|S|}</m>.
	Now
	<md>
	<mrow> (\mu_1 * 1)(n) \amp = \sum_{d \mid n} \mu_1(d) </mrow>
	<mrow> \amp = \sum_{S \subseteq [k]} (-1)^{|S|} </mrow>
	<mrow> \amp = \sum_{j = 0}^k \binom{k}{j} (-1)^j </mrow>
	<mrow> \amp = (1-1)^k </mrow>
	<mrow> \amp = 0 </mrow>
	<mrow> \amp = e(n) </mrow>
	</md>.
  This shows that <m>\mu_1 * 1 = e</m>, and hence <m>\mu_1 = \mu_4</m>,
  as claimed.
	</p>

	</proof>
  
  <proof>
  <title>Alternative proof of <m>\mu_1=\mu_4</m></title>
  <p>
  We know that the arithmetic functions <m>1(n) = 1</m> and <m>e</m>
  are multiplicative (in fact completely multiplicative).
  In addition <m>\mu_1</m> is multiplicative
  (although not completely multiplicative) (exercise).
  Therefore <m>\mu_1 * 1</m> is multiplicative by
  <xref ref="theorem-dirichlet-product-of-multiplicative-functions" />.
  We compute the value
  <md>
  <mrow> (\mu_1 * 1)(p^a) \amp = \mu_1(1) + \mu_1(p) + \mu_1(p^2) + \mu_1(p^3) + \dotsb + \mu_1(p^a) </mrow>
  <mrow> \amp = 1 - 1 + 0 + 0 + \dotsb + 0 </mrow>
  <mrow> \amp = 0 </mrow>
  <mrow> \amp = e(p^a) </mrow>
  </md>.
  This shows that <m>(\mu_1 * 1)(p^a) = e(p^a)</m> for every prime
  power <m>p^a</m>.
  Since both <m>\mu_1 * 1</m> and <m>e</m> are multiplicative,
  it follows that <m>\mu_1 * 1 = e</m>.
  </p>
  </proof>
	
	
	<definition>
	The function <m>\mu_1=\mu_2=\mu_3=\mu_4</m> defined in the above theorem
	is called the <term>Möbius function</term>
	and we henceforth denote it by <m>\mu</m>.
	</definition>

	
  
  </subsection>
	
	
	<subsection>
	<title>Möbius function and Dirichlet product</title>
	
	<p>
	We have seen that <m>\mu * 1 = e</m>.
	Therefore if <m>f</m> and <m>g</m> are any arithmetic functions
	such that <m>f * 1 = g</m>, then <m>f = g * \mu</m>.
	This is called <em>Möbius inversion</em>.
	</p>
	
	<theorem>
	<title>Möbius inversion</title>
	<statement>
	<m>f * 1 = g</m> if and only if <m>f = g * \mu</m>.
	That is,
	<men> g(n) = \sum_{d \mid n} f(d) </men>
	if and only if
	<men> f(n) = \sum_{d \mid n} g(d) \mu\left(\frac{n}{d}\right) </men>.
	</statement>
  <proof>
  Exercise.
  </proof>
  </theorem>
  
  
  <p>
  For example we have <m> \phi * 1 = N </m>,
  and therefore <m> \phi = N * \mu </m>:
  <corollary>
  <statement>
  For all <m>n \geq 1</m>,
  <m>\phi(n) = \sum_{d \mid n} d \mu\left(\frac{n}{d} \right)</m>.
  </statement>
  </corollary>
  (As an exercise, how does this relate to our earlier result
  <m>\phi(n) = n \prod_{p \mid n} (1 - 1/p)</m>?)
  </p>
  
  <p>
  This gives another proof that <m>\phi</m> is multiplicative:
  Since <m>\phi = N * \mu</m>, and <m>N</m> and <m>\mu</m> are
  multiplicative,
  <xref ref="theorem-dirichlet-product-of-multiplicative-functions" />
  shows that <m>\phi</m> is multiplicative.
  </p>
  
  <p>
  Recall that the Von Mangoldt function <m>\Lambda</m> is
  defined by
  <men> \Lambda(n) = \begin{cases}
    \log p, \amp \text{if } n = p^a \\
    0 , \amp \text{otherwise}
    \end{cases}
  </men>
  That is, <m>\Lambda(p^a) = \log p</m> for any prime power
  <m>p^a \gt 1</m>, but <m>\Lambda(1)=0</m> and <m>\Lambda(n) = 0</m>
  when <m>n</m> is not a prime power.
  </p>

  <theorem>
  <statement>
  We have <m>\Lambda * 1 = \log</m>. That is,
  <men>
    \sum_{d \mid n} \Lambda(d) = \log n
  </men>
  for all <m>n \geq 1</m>.
  </statement>
  
  <proof>
  <p>
  For <m>n = 1</m> we have <m>\Lambda(1) = 0</m>,
  so <m>(\Lambda * 1)(1) = 0</m>.
  And <m>\log(1) = 0</m>.
  So <m>(\Lambda * 1)(1) = \log(1)</m>.
  </p>

  <p>
  Let <m>n \gt 1</m> with prime factorization
  <m>n = p_1^{a_1} \dotsm p_k^{a_k}</m>.
  For <m>d \mid n</m>, we have <m>\Lambda(d) = 0</m>
  unless <m>d</m> is a prime power.
  Therefore
  <md>
  <mrow> (\Lambda * 1)(n) \amp = \sum_{d \mid n} \Lambda(d) </mrow>
  <mrow> \amp = \sum_{j = 1}^k \Lambda(p_j) + \Lambda(p_j^2) + \dotsb + \Lambda(p_j^{a_j}) </mrow>
  <mrow> \amp = \sum_{j = 1}^k \log(p_j) + \log(p_j) + \dotsb + \log(p_j) \qquad (a_j \text{ terms}) </mrow>
  <mrow> \amp = \sum_{j = 1}^k a_j \log(p_j) </mrow>
  <mrow> \amp = \log(p_1^{a_1}) + \log(p_2^{a_2}) + \dotsb + \log(p_k^{a_k}) </mrow>
  <mrow> \amp = \log(n) </mrow>
  </md>.
  </p>
  </proof>
  </theorem>
  
  <corollary>
  <statement>
  For <m>n \geq 1</m> we have
  <men>
    \Lambda(n) = \sum_{d \mid n} \mu(d) \log \frac{n}{d}
      = - \sum_{d \mid n} \mu(d) \log d
  </men>.
  </statement>
  
  <proof>
  <p>
  Since <m>\Lambda * 1 = \log</m>, by Möbius inversion we get
  <m>\Lambda = \mu * \log</m>.
  This shows
  <me> \Lambda(n) = \sum_{d \mid n} \mu(d) \log \frac{n}{d} </me>.
  Now,
  <md>
  <mrow> \sum_{d \mid n} \mu(d) \log \frac{n}{d}
         \amp = \sum_{d \mid n} \mu(d) (\log n - \log d) </mrow>
  <mrow> \amp = \sum_{d \mid n} \mu(d) \log n - \sum_{d \mid n} \mu(d) \log d </mrow>
  <mrow> \amp = (\log n) \sum_{d \mid n} \mu(d) - \sum_{d \mid n} \mu(d) \log d </mrow>
  <mrow> \amp = 0 - \sum_{d \mid n} \mu(d) \log d </mrow>
  </md>.
  The reason <m> (\log n) \sum_{d \mid n} \mu(d) = 0 </m> is the following.
  If <m>n \gt 1</m> then <m>\sum_{d \mid n} \mu(d) = 0</m>,
  by the recursive version of the definition of <m>\mu</m>.
  And if <m>n = 1</m> then <m>\log n = 0</m>.
  </p>
  </proof>
  </corollary>
  

	
	</subsection>
	


</section>