<?xml version="1.0" encoding="UTF-8"?>

<section xml:id="sec-af1-dirichlet-product" xmlns:xi="http://www.w3.org/2001/XInclude">
  <title>Dirichlet product</title>
  
  
  <subsection>
  <title>Basic properties of Dirichlet product</title>
  
  <definition>
  Let <m>f,g</m> be arithmetic functions.
  The <term>Dirichlet product</term> of <m>f</m> and <m>g</m>,
  denoted <m>f * g</m>, is the arithmetic function defined by
  <men> (f * g)(n) = \sum_{d \mid n} f(d) g(n/d) = \sum_{de = n} f(d) g(e) </men>
  where the first sum is over positive divisors of <m>n</m>
  and the second sum is over pairs <m>(d,e)</m> of positive integers
  whose product is <m>n</m>.
  </definition>
  
  <example>
  <p> <m> \phi * 1 = N </m>: Here <m>\phi</m> is the Euler totient
  function, <m>1</m> is the function <m>1(n) = 1</m> for all <m>n</m>,
  and <m>N</m> is the function <m>N(n) = n</m> for all <m>n</m>.
  We have shown that <m>\sum_{d \mid n} \phi(d) = n</m>.
  We can rewrite this as <m>\sum_{d \mid n} \phi(d) 1(n/d) = N(n)</m>,
  where the left hand side is <m>(\phi * 1)(n)</m>. This shows
  that <m>\phi * 1 = N</m> as claimed. </p>
  </example>


  <p>
  Other notable operations on arithmetic functions include:
  <ol>
  <li> The sum: <m>(f+g)(n) = f(n)+g(n)</m> </li>
  <li> The pointwise product: <m> (fg)(n) = f(n) g(n)</m> </li>
  <li> The composition: <m> (f \circ g)(n) = f(g(n))</m>
    (assuming <m>g</m> has values in <m>\bbN</m>, the domain of <m>f</m>) </li>
  <li> The Cauchy product, defined by <m> \sum_{d=0}^n f(d)g(n-d) </m>.
    (I'm not sure if there is a common notation for the Cauchy product.) </li>
  </ol>
  </p>
  
  <theorem>
  <statement>
  The Dirichlet product is associative, commutative, and distributes over the sum.
  The function <m>e</m> (defined by <m>e(n)=1</m> if <m>n=1</m>,
  otherwise <m>e(n)=0</m>) is an identity for the Dirichlet product,
  that is, <m>f*e = f</m> for any arithmetic function <m>f</m>.
  </statement>
  
  <proof>
  <p> For associativity:
  <md>
  <mrow> (f*(g*h))(n) \amp = \sum_{d_1 e = n} f(d_1) (g*h)(e) </mrow>
  <mrow> \amp = \sum_{d_1 e = n} f(d_1) \sum_{d_2 d_3 = e} g(d_2) h(d_3) </mrow>
  <mrow> \amp = \sum_{d_1 d_2 d_3 = n} f(d_1) g(d_2) h(d_3) </mrow>
  <mrow> \amp = \sum_{c d_3 = n} \left( \sum_{d_1 d_2 = c} f(d_1) g(d_2) \right) h(d_3) </mrow>
  <mrow> \amp = \sum_{c d_3 = n} (f*g)(c) h(d_3) </mrow>
  <mrow> \amp = ((f*g)*h)(n) </mrow>
  </md>
  </p>
  
  <p> For commutativity:
  <md>
  <mrow> (f*g)(n) \amp = \sum_{de = n} f(d) g(e) </mrow>
  <mrow> \amp = \sum_{ed = n} g(e) f(d) </mrow>
  <mrow> \amp = (g*f)(n) </mrow>
  </md>
  </p>
  
  <p> Distributivity is left as an exercise. </p>
  
  <p> Let <m>f</m> be any arithmetic function. Then
  <men> (f*e)(n) = \sum_{d \mid n} f(d) e(n/d) = f(n) e(n/n) = f(n) </men>,
  since <m>e(n/d) = 0</m> for all <m>d</m> other than <m>d=n</m>.
  So <m>f*e = f</m>. </p>
  </proof>
  </theorem>
  
  <theorem>
  <statement> Let <m>f</m> be an arithmetic function.
  There exists a Dirichlet inverse <m>g</m> such that <m>f*g = e</m>
  if and only if <m>f(1) \neq 0</m>.
  If <m>f(1) \neq 0</m>, then <m>g</m> is defined recursively by
  <m>g(1) = \frac{1}{f(1)}</m> and for <m>n \gt 1</m>,
  <men> g(n) = -\frac{1}{f(1)} \sum_{1 \lt d \mid n} f(d)g(n/d) </men>.
  </statement>
  
  <proof>
  <p> If <m>f*g = e</m> then <m>f(1)g(1) = e(1) = 1</m>, so <m>f(1) \neq 0</m>.
  The converse direction is left as an exercise. </p>
  </proof>
	</theorem>
	
	</subsection>
  
  <subsection>
  <title>Dirichlet product of multiplicative functions</title>
  
  <theorem>
  <statement> If <m>f,g</m> are both multiplicative,
  then so is <m> f * g </m>. </statement>
  
  <proof>
  <p> Suppose <m>(n_1,n_2) = 1</m>.
  Observe that if <m>de = n_1 n_2</m> then there exist factorizations
  <m>d = d_1 d_2</m>, <m>e = e_1 e_2</m>, such that <m>d_1 e_1 = n_1</m>
  and <m>d_2 e_2 = n_2</m>.
  (Simply, <m>d_1</m> is the product of prime factors that are in <m>d</m>
  and <m>n_1</m>, <m>d_2</m> is the product of prime factors that are in
  <m>d</m> and <m>n_2</m>, and so on.) 
  Observe that in this factorization, <m>(d_1,d_2) = (e_1,e_2) = 1</m>. </p>
  
  <p> Now we have
  <md>
  <mrow> (f*g)(n_1 n_2) \amp = \sum_{de = n_1 n_2} f(d) g(e) </mrow>
  <mrow> \amp = \sum_{d_1 d_2 e_1 e_2 = n_1 n_2} f(d_1 d_2) g(e_1 e_2) </mrow>
  <mrow> \amp = \sum_{d_1 e_1 = n_1} \sum_{d_2 e_2 = n_2} f(d_1) f(d_2) g(e_1) g(e_2) </mrow>
  <mrow> \amp = \left( \sum_{d_1 e_1 = n_1} f(d_1) g(e_1) \right)
  	\left( \sum_{d_2 e_2 = n_2} f(d_2) g(e_2) \right) </mrow>
  <mrow> \amp = (f*g)(n_1) (f*g)(n_2) </mrow>
  </md>.
  This shows that <m>f*g</m> is multiplicative.
  </p>
  </proof>
  </theorem>
	
	<corollary>
	<statement> For all <m>s</m>, <m>\sigma_s</m> is multiplicative. </statement>
	
	<proof>
	<p> Let <m>g(n) = n^s</m>, so <m>g</m> is multiplicative
	(in fact, completely multiplicative).
	Then <m>\sigma_s = g * 1</m> where <m>1</m> denotes the arithmetic function
	<m>1(n) = 1</m> for all <m>n</m>.
	Here <m>1</m> is completely multiplicative.
	Since <m>g</m> and <m>1</m> are multiplicative, so is <m>\sigma_s</m>. </p>
	</proof>
	</corollary>
	
	<remark>
	<p> Even if both <m>f</m> and <m>g</m> are completely multiplicative,
	in general <m>f*g</m> is only multiplicative, not necessarily completely
	multiplicative.
	For example let <m>f = g = 1</m>,
	then <m>(f*g)(n) = \sum_{d \mid n} 1 = d(n) = \sigma_0(n)</m>,
	the number of positive divisors of <m>n</m>.
	This is multiplicative but not completely multiplicative,
	for example <m>d(4) = 3 \neq d(2)^2</m>. </p>
	</remark>
	
	<theorem>
	<statement> Let <m>f,g</m> be arithmetic functions.
	If <m>g</m> and <m>f*g</m> are multiplicative, then so is <m>f</m>. </statement>
	
	<proof>
	<p>
	First of all we have <m>(f*g)(1) = 1</m> and <m>g(1) = 1</m> since
	<m>f*g</m> and <m>g</m>are multiplicative.
	By definition of Dirichlet product, <m>(f*g)(1) = f(1)g(1)</m>.
	Therefore <m>f(1) = 1</m>.
	We have <m>f(1 \cdot 1) = 1</m>, that is, <m>f(mn) = 1</m>
	for <m>m=n=1</m>.
	</p>
	
	<p> We will prove the following statement by induction on <m>N</m>:
	<m>f(mn) = f(m)f(n)</m>
	for all <m>m,n</m> such that <m>(m,n)=1</m> and <m>mn \leq N</m>.
	We have seen that this holds for <m>N=1</m>.
	Suppose inductively that it holds for <m>N-1</m>,
	and suppose <m>m,n</m> are positive integers such that
	<m>(m,n)=1</m> and <m>mn=N</m>.
	Since <m>f*g</m> is multiplicative we have
	<md>
	<mrow> (f*g)(mn) \amp = \sum_{d \mid mn} f(d) g(\frac{mn}{d}) </mrow>
	<mrow> \amp = \sum_{d \mid m, e \mid n} f(de) g(\frac{mn}{de}) </mrow>
	<mrow> \amp = \sum_{d \mid m, e \mid n, de \lt mn} f(de) g(\frac{mn}{de}) + f(mn)g(1) </mrow>
	<mrow> \amp = \sum_{d \mid m, e \mid n, de \lt mn} f(d)f(e)g(\frac{m}{d})g(\frac{n}{d}) + f(mn) </mrow>
	<mrow> \amp = \left( \sum_{d \mid m} f(d)g(\frac{m}{d}) \right)
	  \left( \sum_{e \mid n} f(e)g(\frac{n}{e}) \right) - f(m)f(n) + f(mn) </mrow>
	<mrow> \amp = (f*g)(m) (f*g)(n) - f(m)f(n) + f(mn) </mrow>
	<mrow> \amp = (f*g)(mn) - f(m)f(n) + f(mn) </mrow>
	</md>.
	Here we use that <m>f(de) = f(d)f(e)</m> for <m>de \lt mn</m>,
	where <m>(d,e)=1</m> since <m>d \mid m</m> and <m>e \mid n</m>;
	we use that <m>(m/d,n/e) = 1</m> and that <m>g</m> is multiplicative;
	at the end we use that <m>f*g</m> is multiplicative.
	</p>
	
	<p>
	It follows that <m>f(mn) = f(m)f(n)</m>.
  </p>
	</proof>
	</theorem>
	
	<corollary>
	<statement>
	If <m>f</m> is multiplicative then its Dirichlet inverse <m>f^{-1}</m>
	is also multiplicative.
	</statement>
  
  <proof>
  <p> Both <m>f</m> and <m>f*f^{-1} = e</m> are multiplicative. </p>
  </proof>
  </corollary>
  
  <corollary>
  <statement>
  The set of arithmetic functions <m>f</m> with <m>f(1) \neq 0</m>
  is an abelian group under Dirichlet product.
  The subset consisting of multiplicative functions is a subgroup.
  </statement>
  </corollary>
  
  </subsection>
  
  <subsection>
  <title>Explanation of Dirichlet product</title>
  
  <definition>
  <p> A <term>power series</term> centered at <m>c</m>
  is an infinite sum
  <men> f(z) = \sum_{k=0}^{\infty} a_k (z-c)^k </men>.
  The <m>a_k</m> are the <term>coefficients</term> of the power series.
  This sum defines a function of <m>z</m> provided that it converges. </p>
  
  <p> A <term>Dirichlet series</term> is an infinite sum
  <men> f(s) = \sum_{n=1}^{\infty} \frac{a_n}{n^s} </men>.
  Again, the <m>a_n</m> are <term>coefficients</term> of the
  Dirichlet series. The sum defines a function of <m>s</m>
  provided that it converges. </p>
  </definition>
  
  <p> Multiplication of power series corresponds to the Cauchy product
  of coefficients, and multiplication of Dirichlet series corresponds
  to the Dirichlet product of coefficients. </p>
  
  <p> Let us multiply two power series:
  <md>
  <mrow>
    (a_0 + a_1 z + \amp a_2 z^2 + a_3 z^3 + \dotsb) (b_0 + b_1 z + b_2 z^2 + b_3 z^3 + \dotsb)
  </mrow>
  <mrow>
    \amp = (a_0 b_0) + (a_0 b_1 + a_1 b_0) z + (a_0 b_2 + a_1 b_1 + a_2 b_0) z^2
  </mrow>
  <mrow>
     \amp \quad + (a_0 b_3 + a_1 b_2 + a_2 b_1 + a_3 b_0) z^3 + \dotsb
  </mrow>
  </md>
  That is,
  <men>
    \left( \sum a_i z^i \right) \left( \sum b_j z^j \right)
    = \sum_{i,j} a_i b_j z^{i+j}
    = \sum_k \left( \sum_{i+j = k} a_i b_j \right) z^k
  </men>
  This shows that the product of power series with sequences of coefficients
  <m>(a_i)</m> and <m>(b_j)</m> is given by the power series
  with coefficients given by the Cauchy product of
  <m>(a_i)</m> and <m>(b_j)</m>.
  </p>
  
  <p> Similarly, the Dirichlet product corresponds to multiplication
  of Dirichlet series. Let us multiply two Dirichlet series:
  <md>
  <mrow>
    \Big( \frac{a_1}{1^s} + \frac{a_2}{2^s} + \amp \frac{a_3}{3^s} + \frac{a_4}{4^s} + \dotsb \Big)
    \Big( \frac{b_1}{1^s} + \frac{b_2}{2^s} + \frac{b_3}{3^s} + \frac{b_4}{4^s} + \dotsb \Big)
  </mrow>
  <mrow>
    \amp = \frac{a_1 b_1}{1^s 1^s} + \frac{a_1 b_2}{1^s 2^s} + \frac{a_1 b_3}{1^s 3^s} + \frac{a_1 b_4}{1^s 4^s} + \dotsb
  </mrow>
  <mrow>
    \amp \quad + \frac{a_2 b_1}{2^s 1^s} + \frac{a_2 b_2}{2^s 2^s} + \frac{a_2 b_3}{2^s 3^s} + \frac{a_2 b_4}{2^s 4^s} + \dotsb
  </mrow>
  <mrow>
    \amp \quad + \frac{a_3 b_1}{3^s 1^s} + \frac{a_3 b_2}{3^s 2^s} + \frac{a_3 b_3}{3^s 3^s} + \frac{a_3 b_4}{3^s 4^s} + \dotsb
  </mrow>
  <mrow>
    \amp = \frac{a_1 b_1}{1^s} + \frac{a_1 b_2}{2^s} + \frac{a_1 b_3}{3^s} + \frac{a_1 b_4}{4^s} + \dotsb
  </mrow>
  <mrow>
    \amp \quad + \frac{a_2 b_1}{2^s} + \frac{a_2 b_2}{4^s} + \frac{a_2 b_3}{6^s} + \frac{a_2 b_4}{8^s} + \dotsb
  </mrow>
  <mrow>
    \amp \quad + \frac{a_3 b_1}{3^s} + \frac{a_3 b_2}{6^s} + \frac{a_3 b_3}{9^s} + \frac{a_3 b_4}{12^s} + \dotsb
  </mrow>
  <mrow>
    \amp = \frac{a_1 b_1}{1^s} + \frac{a_1 b_2 + a_2 b_1}{2^s} + \frac{a_1 b_3 + a_3 b_1}{3^s}
      + \frac{a_1 b_4 + a_2 b_2 + a_4 b_1}{4^s} + \dotsb
  </mrow>
  </md>
  In general,
  <men>
    \left( \sum \frac{a_m}{m^s} \right) \left( \sum \frac{b_n}{n^s} \right)
    = \sum_{m,n} \frac{a_m b_n}{(mn)^s}
    = \sum_k \frac{ \sum_{mn = k} a_m b_n }{ k^s }
    = \sum_k \frac{(a*b)_k}{k^s}
  </men>
  </p>
  
  </subsection>
  


</section>